especialize now must ecplicitely cite created evars.
Still looking for a way to have a "default mode" where all variables
needed to *type* the premised to be proved are evarized.

For not we do

especialize X with x,y,z at 1,2,3.

And we get errors if we forget a variable.

LibHyps/LibEspecialize.v
@@ -1,14 +1,33 @@
+
+Require Import LibHyps.LibHypsTactics.
+
+(* debug *)
+Module Prgoal_Notation.
+  Ltac pr_goal :=
+    match goal with
+      |- ?g =>
+        let allh := harvest_hyps revert_clearbody_all in
+        (* let allh := all_hyps in *)
+        idtac allh " ⊢ " g
+    end.
+End Prgoal_Notation.
+
 Require Import Arith.
 (* The tactics in this file use the folowing pattern, that consists in
    refining a new evar goal until being in the right scope to prove
    the premise. *)
-(* 
+(*
 Lemma foo: forall x y : nat, (forall n m p :nat, n < m -> n <= m -> p > 0 -> False) -> False.
 Proof.
   intros x y H. 
   (* On veut prouver le n <= m comme conséquence du n < m dans H. *)
   (* On crée un but dont le type n'est pas connu, et on raffine pour
      être dans le bon environnement. *)
+
+  assert (forall n m p : nat, n < m -> n <= m).
+  { admit. }
+  pose proof (fun (n m p : nat) (h:n < m) => (H n m p h (H0 n m p h))).
+
   let ev := open_constr:(_) in
   assert (ev) as h.
   { refine (fun (n m p:nat) (h:n < m) => _).
@@ -21,256 +40,625 @@ Admitted.
 
 (* Describing how each arg of a hypothesis must be treated: either
    requantify it, or evarize it, or requantify but don't use it in
-   premise proofs (not sure this is needed). We don't use list for
-   cosmetic reasons: no need for nil (since the list is non empty),
-   and avoid using lists. *)
+   premise proofs (not sure this is needed) finally make it a subgoal.
+   We don't use list for cosmetic reasons: no need for nil (since the
+   list is non empty). *)
 Inductive spec_args : Type :=
-  ConsQuantif: spec_args -> spec_args
-| ConsEvar: spec_args -> spec_args
-| ConsIgnore: spec_args -> spec_args
-| ConsSubGoal: spec_args -> spec_args
-| SubGoalEnd: spec_args.
-
-(* List storing heterogenous terms, for storing (tele(scopes). A
-   simple product could also be used. *)
-Inductive Depl :=
-| DNil: Depl
-| DCons: forall (A:Type) (x:A), Depl -> Depl.
-
-Declare Scope specialize_scope.
-Delimit Scope specialize_scope with spec.
-Local Open Scope specialize_scope.
+  ConsQuantif: spec_args -> spec_args (* re-quantify *)
+| ConsEvar: spec_args -> spec_args    (* make it an evar *)
+| ConsIgnore: spec_args -> spec_args  (* gnore it (useless?) *)
+| ConsSubGoal: spec_args -> spec_args (* make it a subgoal *)
+| SubGoalEnd: spec_args.              (* make it a subgoal, end of list. *)
 
 
-(* builds the application of c to each element of l (in reversed
+Inductive int_spec_args: Type :=
+| ConsEVAR: nat -> int_spec_args -> int_spec_args
+| ConsGOAL: nat -> int_spec_args -> int_spec_args
+| FinalGOAL: nat -> int_spec_args.
+
+
+Declare Scope especialize_scope.
+Delimit Scope especialize_scope with espec.
+(* Local Open Scope especialize_scope. *)
+
+Declare Scope especialize_using_scope.
+Delimit Scope especialize_using_scope with euspec.
+(* Local Open Scope especialize_using_scope. *)
+
+Module SpecNotation.
+
+  Infix "?::" := ConsEVAR (at level 60, right associativity) : especialize_scope.
+  Infix "#::" := ConsGOAL (at level 60, right associativity) : especialize_scope.
+  Notation "## X" := (FinalGOAL X) (at level 60) : especialize_scope.
+
+  Notation "! X" := (ConsQuantif X) (at level 100) : especialize_using_scope.
+  Notation "? X" := (ConsEvar X) (at level 100) : especialize_using_scope.
+  Notation "# X" := (ConsSubGoal X) (at level 100) : especialize_using_scope.
+  Notation "##" := (SubGoalEnd) (at level 100) : especialize_using_scope.
+
+  Ltac interp_num min l :=
+    lazymatch l with
+      nil => fail
+    | FinalGOAL ?min' =>
+        match min with
+          min' => constr:(SubGoalEnd)
+        | _ => 
+            let lres := interp_num (S min) l in
+            constr:(ConsQuantif lres)
+        end
+    | ConsGOAL ?min' ?l' =>
+        match min with
+          min' =>
+            let lres := interp_num (S min) l' in
+            constr:(ConsSubGoal lres)
+        | _ => 
+            let lres := interp_num (S min) l in
+            constr:(ConsQuantif lres)
+        end
+    | ConsEVAR ?min' ?l' =>
+        match min with
+          min' =>
+            let lres := interp_num (S min) l' in
+            constr:(ConsEvar lres)
+        | _ => 
+            let lres := interp_num (S min) l in
+            constr:(ConsQuantif lres)
+        end
+    end.
+
+End SpecNotation.
+Import SpecNotation.
+
+  (* builds the application of c to each element of l (in reversed
    order). apply t [t1;t2;t3] => (t t3 t2 t1) *)
-Ltac list_apply c l :=
-  match l with
-    DNil => c
-  | DCons _ ?x ?l' =>
-      let inside := list_apply c l' in
-      let res := constr:(ltac:(exact (inside x))) in
-      res
-  end.
+  Ltac list_apply c l :=
+    match l with
+      DNil => c
+    | DCons _ ?x ?l' =>
+        let inside := list_apply c l' in
+        let res := constr:(ltac:(exact (inside x))) in
+        res
+    end.
 
-(* - We start from a goal evar EV with no typing constraint.
+  Ltac refine_hd h largs :=
+    match largs with
+    | SubGoalEnd =>
+        match type of h with
+        | (forall x:?t, _) =>
+            (* create the user subgoal *)
+            let x' := fresh x in
+            unshelve (evar(x':t); exact (h x'))
+        end
+    | ConsQuantif ?largs' => 
+        match type of h with
+        | (forall x:?t, _) =>
+            let x':= fresh x in
+            refine (fun x': t => _);
+            specialize (h x');
+            refine_hd h largs'
+        end
+    (* Fallback to evar creation *)
+    (* | ConsQuantif ?largs' => refine_hd h (ConsEvar largs') *)
+    | ConsEvar ?largs' => 
+        match type of h with
+        | (forall x:?t, _) =>
+            let x' := fresh x in
+            evar(x':t);
+            specialize (h x');
+            subst x';
+            refine_hd h largs'
+        end
+    | ConsSubGoal ?largs' =>
+        match type of h with
+        | (forall x:?t, _) =>
+            let x' := fresh x in
+            unshelve (evar(x':t));[
+                clear h 
+              | specialize (h x');
+                refine_hd h largs']
+        end
+    end.
 
-    h: forall x y z, P x -> ...
-    ========================
-    ?EV
 
-    subgoal 2
-    h: forall x y z, P x -> ...
-    ========================
-    old goal
-    
+  Ltac refine_premise_hd h largs :=
+    match largs with
+    | SubGoalEnd =>
+        match type of h with
+        | (forall x:?t, _) =>
+            (* create the user subgoal *)
+            let x' := fresh x in
+            unshelve (evar(x':t); exact x')
+        end
+    | ConsQuantif ?largs' => 
+        match type of h with
+        | (forall x:?t, _) =>
+            let x':= fresh x in
+            refine (fun x': t => _);
+            specialize (h x');
+            refine_premise_hd h largs'
+        end
+    (* Fallback to evar creation *)
+    (* | ConsQuantif ?largs' => refine_premise_hd h (ConsEvar largs') *)
+    | ConsEvar ?largs' => 
+        match type of h with
+        | (forall x:?t, _) =>
+            let x' := fresh x in
+            evar(x':t);
+            specialize (h x');
+            subst x';
+            refine_premise_hd h largs'
+        end
+    | ConsSubGoal ?largs' =>
+        match type of h with
+        | (forall x:?t, _) =>
+            let x' := fresh x in
+            unshelve (evar(x':t));[
+                clear h 
+              | specialize (h x');
+                refine_premise_hd h largs']
+        end
+    end.
 
-  - We refine is to have the same products at head than h, until we
-    reach the aimed hypothesis
 
-    h: P x -> ...
-    x: ...   y: ...   z: ...
-    ========================
-    ?EV
-
-  - then we do 2 things
-    - create a goal USERGOAL for this hyp
-    - conclude EV (and fix its type) by applying h to USERGOAL
-
-    subgoal 1
-    x: ...   y: ...   z: ...
-    ==========================
-    P x
-
-    subgoal 2:
-    h: forall x y z, P x -> ...
-    hEV: forall x y z, ...
-    ==========================
-    old goal
-
-   Refines a non specified goal (an evar) to prove the specialized
-   version of h. The idea is to use (fun x y z => (?ev x y z)) as the
-   argument being instnaciated, where ?ev will be the new goal
-
- larg is the specidication of what to do with each arg, larg2 is the
-   accumulator *)
-Ltac refine_hd h largs largs2 :=
-  match largs with
-  | SubGoalEnd => match type of h with
-                  | (forall x:?t, _) =>
-                      let h' := fresh h in
-                      (* create the user subgoal *)
-                      assert(t) as h'
-                      ;[ clear h
-                       | exact (h h')
-                         (*let res := list_apply h' largs2 in
-                  exact (h res) *) ]  
-                  end
-  | ConsQuantif ?largs' => 
-      match type of h with
-      | (forall x:?t, _) =>
-          (* let y:= fresh x in *)
-          (* intro y; *)
-          refine (fun x: t => _);
-          specialize (h x);
-          refine_hd h largs' constr:(DCons _ x largs2)
-      end
-  | ConsEvar ?largs' => 
-      match type of h with
-      | (forall x:?t, _) =>
-          (* morally this evar is of type t, don't know how to enforce this
-             without having an ugly cast in goals *)
-          let ev1 := open_constr:(_:t) in
-          refine (let x:= ev1 in _);
-          specialize (h x);
-          subst x;
-          refine_hd h largs' largs2
-      end
-  | ConsSubGoal?largs' => match type of h with
-                          | (forall x:?t, _) =>
-                              let h' := fresh h in
-                              (* create the user subgoal *)
-                              assert(t) as h'
-                              ;[ clear h
-                               | exact (h h')
-                                 (*let res := list_apply h' largs2 in
-                                   exact (h res) *) ]   
-                          end
-  end.
-
-(* Precondition: name is already fresh *)
-Global Ltac espec_gen H l name :=
-  (* let l := eval cbn [spec_interp] in (spec_interp args) in   *)
-  (* let h := fresh name in *)
-  (* morally this evar is of type Type, don't know how to enforce this
+  (* Precondition: name is already fresh *)
+  Global Ltac espec_gen H l name :=
+    (* morally this evar is of type Type, don't know how to enforce this
      without having an ugly cast in goals *)
-  let ev1 := open_constr:(_) in
-  assert ev1 as name
-  ; [
-      (refine_hd H l DNil)
-    | ].
-  
-Global Ltac especialize_clear H args :=
-  let temp := fresh H "temp" in
-  espec_gen H args temp;
-  [ | clear H;
-      idtac "ICI: " temp;
-      rename temp into H ].
+    let ev1 := open_constr:(_) in
+    assert ev1 as name
+    ; [
+        (refine_hd H l)
+      | ].
 
-Global Ltac especialize_autoname H args :=
-  let name := fresh H "_inst" in
-  espec_gen H args name.
-
-Global Ltac especialize_clear_autoname H args :=
-  let name := fresh H "_inst" in
-  especialize_autoname H args name.
-
-Module SpecNotation.
-  (* Notation "![ ]!" := DNil (format "![ ]!") : specialize_scope. *)
-  (* Notation "![ x ]!" := (DCons _ x nil) : specialize_scope. *)
-  (* Notation "![ x ; y ; .. ; z ]!" := *)
-    (* (DCons _ x (DCons _ y .. (DCons _ z DNil) ..)) *)
-      (* (format "![ '[' x ;  '/' y ;  '/' .. ;  '/' z ']' ]!") : specialize_scope. *)
-  Notation "! X" := (ConsQuantif X) (at level 100) : specialize_scope.
-  Notation "? X" := (ConsEvar X) (at level 100) : specialize_scope.
-  Notation "# X" := (ConsSubGoal X) (at level 100) : specialize_scope.
-  Notation "#" := (SubGoalEnd) (at level 100) : specialize_scope.
-Module SpecNotation.
-
-Tactic Notation "especialize" constr(H) "at" constr(specarg) "as" ident(idH) :=
-  espec_gen H specarg idH.
-Tactic Notation "especialize"  constr(specarg) "as" constr(H) "at" ident(idH) :=
-  espec_gen H specarg idH.
-
-Tactic Notation "especialize" constr(H) "at" constr(specarg) :=
-  especialize_clear H specarg.
+  Global Ltac eprem_gen H l name :=
+    (* morally this evar is of type Type, don't know how to enforce this
+     without having an ugly cast in goals *)
+    let ev1 := open_constr:(_) in
+    assert ev1 as name
+    ; [
+        (refine_premise_hd H l)
+      | ].
 
 
+  Ltac fresh_unfail H :=
+    match constr:(True) with
+    | _ => fresh H
+    | _ => fresh "H_"
+    end.
+  Global Ltac especialize_clear H args :=
+    (is_var H ; 
+     let temp := fresh_unfail H in
+     espec_gen H args temp; [ .. | clear H; rename temp into H ])
+    + ((assert_fails (is_var(H))) ; 
+       let tempH := fresh_unfail H in
+       specialize H as tempH;
+       let temp := fresh_unfail H in
+       espec_gen tempH args temp).
 
 
-Definition eq_one (i:nat) := i = 1.
+  Global Ltac especialize_named H args name :=
+    (is_var H ; espec_gen H args name)
+    + ((assert_fails (is_var(H))) ; 
+       let tempH := fresh_unfail H in
+       specialize H as tempH;
+       espec_gen tempH args name;
+       [ .. | clear tempH ]).
+
+  Global Ltac epremise_named H args name :=
+    (is_var H ; eprem_gen H args name)
+    + ((assert_fails (is_var(H))) ; 
+       let tempH := fresh_unfail H in
+       specialize H as tempH;
+       eprem_gen tempH args name;
+       [ .. | clear tempH ]).
 
 
-Lemma test_espec: forall x:nat, (forall y:nat,eq_one 2 -> eq_one 3 -> eq_one y -> x=0 -> False) -> True.
+  Global Ltac especialize_autoname H args :=
+    let name := fresh_unfail H in
+    espec_gen H args name.
+
+  Global Ltac especialize_clear_autoname H args :=
+    let name := fresh_unfail H in
+    (* let name := fresh name "_inst" in *)
+    especialize_autoname H args name.
+
+
+  Tactic Notation "especialize" constr(H) "using" constr(specarg) "as" ident(idH) :=
+    especialize_named H specarg idH.
+
+  Tactic Notation "especialize" constr(H) "using" constr(specarg) :=
+    especialize_clear H specarg.
+
+  (* TODO *)
+  Tactic Notation "especialize" constr(H) "using" constr(specarg) ":" ident(hprem) :=
+    especialize_clear H specarg.
+
+  Tactic Notation "assert" "premises" constr(H) "at" constr(specarg) "as" ident(idH) :=
+    let specarg' := SpecNotation.interp_num 1%nat specarg in
+    epremise_named H specarg' idH.
+
+
+  Tactic Notation "especialize" constr(H) "at" constr(specarg) "as" ident(idH) :=
+    let specarg' := SpecNotation.interp_num 1%nat specarg in
+    especialize_named H specarg' idH.
+
+  Tactic Notation "assert" "premises" constr(H) "at" constr(specarg) :=
+    let specarg' := SpecNotation.interp_num 1%nat specarg in
+    let idH := fresh "Hprem" in
+    epremise_named H specarg' idH.
+
+  Tactic Notation "especialize" constr(H) "at" constr(specarg) :=
+    let specarg' := SpecNotation.interp_num 1%nat specarg in
+    especialize_clear H specarg'.
+
+  (* TODO *)
+  Tactic Notation "especialize" constr(H) "at" constr(specarg) ":" ident(hprem) :=
+    let specarg' := SpecNotation.interp_num 1%nat specarg in
+    especialize_clear H specarg'.
+
+
+  (* Tactic Notation "exploit" constr(H) "using" constr(specarg) "as" ident(idH) := *)
+  (* prove_premises H specarg idH. *)
+
+
+
+
+  Ltac check_var H :=
+    (is_var(H))
+    + (assert_fails(is_var(H))
+       ; fail "the term " H "is not a hypothesis. To create a new hypothesis from it, please us 'as <name>'. ").
+
+
+
+  (* SPECIALIZE WITH EVAR(S) *)
+  (* Precondiion: H must already be a hyp at this point. *)
+  Ltac spec_evar H var_name :=
+    check_var(H);
+    let idt := fresh var_name "T" in
+    let id := fresh var_name in
+    evar (idt : Type);
+    evar (id : idt);
+    specialize H with (var_name := id); subst id; subst idt.
+
+  Tactic Notation "specevar" constr(H) "at" ident(i) "as" ident(newH) :=
+    specialize H as newH;
+    spec_evar newH i.
+
+  Tactic Notation "specevar" constr(H) "at" ident(i) "as" "?" :=
+    let newH := fresh "H" in
+    specevar newH at i as newH.
+
+  Ltac create_hyp_if_necessary H :=
+    (assert_fails(is_var(H)); let newH := fresh_unfail H in specialize H as newH)
+    + idtac.
+
+
+  (* Without a name: duplicate only if c is not a hypothesis, otherwise
+   specialize directly on H *)
+  Tactic Notation "specevar" constr(c) "at" ident(i) :=
+    create_hyp_if_necessary c;
+    spec_evar c i.
+
+
+  Definition eq_one (i:nat) := i = 1.
+(*
+Module Using.
+
+Local Open Scope especialize_using_scope.
+
+Lemma test_espec: forall x:nat, x = 1 -> (forall a y z:nat, a = 1 -> y = 1 -> z+y+a = 2 -> z+1 = x -> False) -> x > 1.
 Proof.
-  intros x h_eqone.
-  (* let nme := fresh_robust H "hh" "def" in idtac nme.Definition *)
+  intros x hx h_eqone.
+  (* specevar h_eqone at y. *)
+  especialize h_eqone using (? ? ! # ##).
+  + reflexivity.
+  + reflexivity.
+  + exfalso.
+    apply h_eqone with 0.
+    * reflexivity.
+    * symmetry.
+      assumption.
+Qed.
   
-  especialize h_eqone at (?#) as newH.
-    [ admit | ].  match type of newH with (eq_one 2 -> eq_one y -> x = 0 -> False) => idtac end;
-              match type of h_eqone with forall y : nat, eq_one 2 -> eq_one 3 -> eq_one y -> x = 0 -> False => idtac end].
-  Undo.
-  especialize h_eqone at (!!#) as newH;
-    [ admit | match type of newH with (forall y : nat, eq_one 2 -> eq_one y -> x = 0 -> False) => idtac end;
-              match type of h_eqone with forall y : nat, eq_one 2 -> eq_one 3 -> eq_one y -> x = 0 -> False => idtac end].
-  Undo.
-  especialize h_eqone at (!#) as newH
-  ;[ admit
-   |  match type of newH with  forall y : nat, eq_one 3 -> eq_one y ->  x = 0 -> False => idtac end;
-        match type of h_eqone with forall y : nat, eq_one 2 -> eq_one 3 -> eq_one y -> x = 0 -> False => idtac end].
-
-  Undo.
-  especialize h_eqone at (!!!#) as newH;
-    [ admit | match type of newH with  nat -> eq_one 2 -> eq_one 3 -> x = 0 -> False => idtac end;
-                match type of h_eqone with forall y : nat, eq_one 2 -> eq_one 3 -> eq_one y -> x = 0 -> False => idtac end].
-  Undo.
-
-
-Lemma test_espec: (eq_one 2 -> eq_one 3 -> eq_one 1 -> False) -> True.
+Lemma test_espec': forall x:nat, x = 1 -> (forall a y z:nat, a = 1 -> y = 1 -> z+y+a = 2 -> z+1 = x -> False) -> x > 1.
 Proof.
-  intros h_eqone.
-
-
-  (* let nme := fresh_robust H "hh" "def" in idtac nme.Definition *)
-  pose (c:= !!?#).
-  pose (c:= !!?#!#).
-  especialize h_eqone at (!#) as newH;
-    [ admit | match type of newH with eq_one 2 -> eq_one 1 -> False => idtac end;
-              match type of h_eqone with  eq_one 2 -> eq_one 3 -> eq_one 1 -> False => idtac end].
-  Undo.
-  especialize h_eqone at (?) as newH
-  ;[ admit
-       | match type of newH with  eq_one 3 -> eq_one 1 -> False => idtac end;
-         match type of h_eqone with  eq_one 2 -> eq_one 3 -> eq_one 1 -> False => idtac end].
-
-  Undo.
-  especialize h_eqone at (!!#) as newH;
-    [ admit | match type of newH with eq_one 2 -> eq_one 3 -> False => idtac end;
-              match type of h_eqone with  eq_one 2 -> eq_one 3 -> eq_one 1 -> False => idtac end].
-
-
-
-  especialize (let x:=Nat.le_antisymm in x) at 2 as hhh;
-    [ admit | match type of hhh with _ <= _ -> _ = _ => idtac | _ => fail "Test failed!" end ].
-  Undo.
-
-  especialize (let x:=Nat.le_antisymm in x)as hhh at 2;
-    [ admit | match type of hhh with _ <= _ -> _ = _ => idtac | _ => fail "Test failed!" end ].
-  Undo.
-
-  especialize h_eqone at 2;
-    [ admit | match type of h_eqone with eq_one 2 -> eq_one 1 -> False => idtac end].
-  Undo.
-
-  especialize (let x:=Nat.le_antisymm in x) at 2;
-    [ admit | match goal with |- (_ <= _ -> _ = _) -> True => idtac | _ => fail "Test failed!" end ].
-  Undo.
-
-  especialize h_eqone as ? at 2;
-    [ admit | match type of h_eqone_spec with eq_one 2 -> eq_one 1 -> False => idtac | _ => fail "Test failed!" end;
-              match type of h_eqone with eq_one 2 -> eq_one 3 -> eq_one 1 -> False => idtac | _ => fail "Test failed!" end].
-  Undo.
-  especialize h_eqone at 2 as ? ;
-    [ admit | match type of h_eqone_spec with eq_one 2 -> eq_one 1 -> False => idtac | _ => fail "Test failed!" end;
-              match type of h_eqone with eq_one 2 -> eq_one 3 -> eq_one 1 -> False => idtac | _ => fail "Test failed!" end].
-  Undo.
+  intros x hx h_eqone.
+  (* specevar h_eqone at y. *)
+  especialize h_eqone using (? ? ! # ##) as h_eqonetemp.
+  + reflexivity.
+  + reflexivity.
+  + exfalso.
+    apply h_eqonetemp with 0.
+    * reflexivity.
+    * symmetry.
+      assumption.
+Qed.
   
-  especialize (let x:=Nat.le_antisymm in x) as ? at 2;
-    [ admit | match type of H_spec with _ <= _ -> _ = _ => idtac | _ => fail "Test failed!" end;
-              match type of h_eqone with eq_one 2 -> eq_one 3 -> eq_one 1 -> False => idtac | _ => fail "Test failed!" end].
-  Undo.
 
-  especialize (let x:=Nat.le_antisymm in x) at 2 as ? ;
-    [ admit | match type of H_spec with _ <= _ -> _ = _ => idtac | _ => fail "Test failed!" end;
-              match type of h_eqone with eq_one 2 -> eq_one 3 -> eq_one 1 -> False => idtac | _ => fail "Test failed!" end].
-  Undo.
+Lemma test_espec2: forall x:nat, x = 1 -> (forall a y z:nat, a = 1 -> y = 1 -> z+y+a = 2 -> z+1 = x -> False) -> x > 1.
+Proof.
+  intros x hx h_eqone.
+  (* specevar h_eqone at y. *)
+  especialize h_eqone using (! ? ! ! ##).
+  + reflexivity.
+  + exfalso.
+    apply h_eqone with 1 0.
+    * reflexivity.
+    * reflexivity.
+    * symmetry.
+      assumption.
+Qed.
+  
+
+Lemma test_espec3: forall x:nat, x = 1 -> (forall a y z:nat, a = 1 -> y = 1 -> z+y+a = 2 -> z+1 = x -> False) -> x > 1.
+Proof.
+  intros x hx h_eqone.
+  (* specevar h_eqone at y. *)
+  especialize h_eqone using (! ? ? ! ##).
+  + reflexivity.
+  + exfalso.
+    apply h_eqone with 1.
+    * reflexivity.
+    * instantiate (z:=0). reflexivity.
+    * symmetry.
+      assumption.
+Qed.
+  
+
+Lemma test_espec4: forall x:nat, x = 1 -> (forall a y z:nat, a = 1 -> y = 1 -> z+y+a = 2 -> z+1 = x -> False) -> x > 1.
+Proof.
+  intros x hx h_eqone.
+  (* specevar h_eqone at y. *)
+  especialize h_eqone using (? ? ? ! ##).
+  + reflexivity.
+  + exfalso.
+    apply h_eqone.
+    * reflexivity.
+    * instantiate (z:=0). reflexivity.
+    * symmetry.
+      assumption.
+Qed.
+  
+Lemma test_espec5: forall x:nat, x = 1 -> (forall a y z:nat, a = 1 -> y = 1 -> z+y+a = 2 -> z+1 = x -> False) -> x > 1.
+Proof.
+  intros x hx h_eqone.
+  (* specevar h_eqone at y. *)
+  especialize h_eqone using (? ? ? ##).
+  + reflexivity.
+  + exfalso.
+    apply h_eqone.
+    * reflexivity.
+    * instantiate (z:=0). reflexivity.
+    * symmetry.
+      assumption.
+Qed.
+  
+Lemma test_espec6: forall x:nat, x = 1 -> (forall a y z:nat, a = 1 -> y = 1 -> z+y+a = 2 -> z+1 = x -> False) -> x > 1.
+Proof.
+  intros x hx h_eqone.
+  (* specevar h_eqone at y. *)
+  especialize h_eqone using (? ! ! ##).
+  + reflexivity.
+  + exfalso.
+    apply h_eqone with 1 0.
+    * reflexivity.
+    * reflexivity.
+    * symmetry.
+      assumption.
+Qed.
+
+Lemma test_espec7: forall x:nat, x = 1 -> (forall a y z:nat, a = 1 -> y = 1 -> z+y+a = 2 -> z+1 = x -> False) -> x > 1.
+Proof.
+  intros x hx h_eqone.
+  (* specevar h_eqone at y. *)
+  especialize h_eqone using (? ! ? # ! ! ##).
+  + reflexivity.
+  + rewrite hx.
+    instantiate (z:=0).
+    reflexivity.
+  + exfalso.
+    apply h_eqone with 1.
+    * reflexivity.
+    * reflexivity.
+Qed.
+
+Lemma test_espec8: forall x:nat, x = 1 -> (forall a y z:nat, a = 1 -> y = 1 -> z+y+a = 2 -> z+1 = x -> False) -> x > 1.
+Proof.
+  intros x hx h_eqone.
+  (* specevar h_eqone at y. *)
+  especialize h_eqone using (? ! ! # ! ! ##).
+  + reflexivity.
+  + subst.
+    rewrite Nat.add_comm in x2.
+    cbn in x2.
+    injection x2;intro ;assumption.
+  + exfalso.
+    apply h_eqone with 1 0.
+    * reflexivity.
+    * reflexivity.
+Qed.
+
+Lemma test_espec9: forall x:nat, x = 1 -> (forall a y z:nat, a = 1 -> y = 1 -> z+y+a = 2 -> z+1 = x -> False) -> x > 1.
+Proof.
+  intros x hx h_eqone.
+  (* specevar h_eqone at y. *)
+  especialize h_eqone using (! ! ! # ! ! ##).
+  + subst.
+    Fail
+      (* this should fail if there are only nat hyps: *)
+      ltac:(match goal with
+            | H: ?t |- a = 1 =>
+                match t with
+                  nat => fail 1
+                | _ => idtac "remaining hyp: " H ":" t 
+                end
+            end).
+Abort.
+
+End Using. *)
+
+
+Import SpecNotation.
+  Module At.
+    Module Using.
+      Import List.ListNotations.
+      Open Scope list_scope.
+
+      Close Scope autonaming_scope.
+      Open Scope especialize_scope.
+      Lemma test_espec: forall x:nat, x = 1 -> (forall a y z:nat, a = 1 -> y = 1 -> z+y+a = 2 -> z+1 = x -> False) -> x > 1.
+      Proof.
+        intros x hx h_eqone.
+        (* specevar h_eqone at y. *)
+        (* especialize h_eqone at (ConsEVAR 1 (ConsEVAR 2 (ConsGOAL 4 (FinalGOAL 5)))). *)
+        assert premises h_eqone at (2?::##5) as h.
+        + reflexivity.
+        + exfalso.
+          eapply h_eqone with (z:=0);eauto.
+          subst.
+          reflexivity.
+Qed.
+
+
+
+Lemma foo: False.
+Proof.
+  (* specialize (le_sind 0) as h. *)
+  (* Set Ltac Debug. *)
+  especialize (le_sind 0)  at (1?:: ##2) as h'.
+  (* Set Ltac Debug. *)
+  especialize (le_sind 0) at (1?:: ##2) as h.  ? P.  as hh : h.
+  { admit. }
+  especialize min_l at 1 as ? : ?.
+  { apply (le_n O). }
+  
+  especialize H at 1 as hh : h.
+  { reflexivity. }
+  match type of h with False => idtac "OK" | _ => fail end.
+  assumption.
+Qed.
+*)
+
+
+Lemma test_espec2: forall x:nat, x = 1 -> (forall a y z:nat, a = 1 -> y = 1 -> z+y+a = 2 -> z+1 = x -> False) -> x > 1.
+Proof.
+  intros x hx h_eqone.
+  (* specevar h_eqone at y. *)
+  especialize h_eqone using (! ? ! ! ##).
+  + reflexivity.
+  + exfalso.
+    apply h_eqonetemp with 1 0.
+    * reflexivity.
+    * reflexivity.
+    * symmetry.
+      assumption.
+Qed.
+  
+
+Lemma test_espec3: forall x:nat, x = 1 -> (forall a y z:nat, a = 1 -> y = 1 -> z+y+a = 2 -> z+1 = x -> False) -> x > 1.
+Proof.
+  intros x hx h_eqone.
+  (* specevar h_eqone at y. *)
+  especialize h_eqone using (! ? ? ! ##).
+  + reflexivity.
+  + exfalso.
+    apply h_eqonetemp with 1.
+    * reflexivity.
+    * instantiate (z:=0). reflexivity.
+    * symmetry.
+      assumption.
+Qed.
+  
+
+Lemma test_espec4: forall x:nat, x = 1 -> (forall a y z:nat, a = 1 -> y = 1 -> z+y+a = 2 -> z+1 = x -> False) -> x > 1.
+Proof.
+  intros x hx h_eqone.
+  (* specevar h_eqone at y. *)
+  especialize h_eqone using (? ? ? ! ##).
+  + reflexivity.
+  + exfalso.
+    apply h_eqonetemp.
+    * reflexivity.
+    * instantiate (z:=0). reflexivity.
+    * symmetry.
+      assumption.
+Qed.
+  
+Lemma test_espec5: forall x:nat, x = 1 -> (forall a y z:nat, a = 1 -> y = 1 -> z+y+a = 2 -> z+1 = x -> False) -> x > 1.
+Proof.
+  intros x hx h_eqone.
+  (* specevar h_eqone at y. *)
+  especialize h_eqone using (? ? ? ##).
+  + reflexivity.
+  + exfalso.
+    apply h_eqonetemp.
+    * reflexivity.
+    * instantiate (z:=0). reflexivity.
+    * symmetry.
+      assumption.
+Qed.
+  
+Lemma test_espec6: forall x:nat, x = 1 -> (forall a y z:nat, a = 1 -> y = 1 -> z+y+a = 2 -> z+1 = x -> False) -> x > 1.
+Proof.
+  intros x hx h_eqone.
+  (* specevar h_eqone at y. *)
+  especialize h_eqone using (? ! ! ##).
+  + reflexivity.
+  + exfalso.
+    apply h_eqonetemp with 1 0.
+    * reflexivity.
+    * reflexivity.
+    * symmetry.
+      assumption.
+Qed.
+
+Lemma test_espec7: forall x:nat, x = 1 -> (forall a y z:nat, a = 1 -> y = 1 -> z+y+a = 2 -> z+1 = x -> False) -> x > 1.
+Proof.
+  intros x hx h_eqone.
+  (* specevar h_eqone at y. *)
+  especialize h_eqone using (? ! ? # ! ! ##).
+  + reflexivity.
+  + rewrite hx.
+    instantiate (z:=0).
+    reflexivity.
+  + exfalso.
+    apply h_eqonetemp with 1.
+    * reflexivity.
+    * reflexivity.
+Qed.
+
+Lemma test_espec8: forall x:nat, x = 1 -> (forall a y z:nat, a = 1 -> y = 1 -> z+y+a = 2 -> z+1 = x -> False) -> x > 1.
+Proof.
+  intros x hx h_eqone.
+  (* specevar h_eqone at y. *)
+  especialize h_eqone using (? ! ! # ! ! ##).
+  + reflexivity.
+  + subst.
+    rewrite Nat.add_comm in x2.
+    cbn in x2.
+    injection x2;intro ;assumption.
+  + exfalso.
+    apply h_eqonetemp with 1 0.
+    * reflexivity.
+    * reflexivity.
+Qed.
+
+Lemma test_espec9: forall x:nat, x = 1 -> (forall a y z:nat, a = 1 -> y = 1 -> z+y+a = 2 -> z+1 = x -> False) -> x > 1.
+Proof.
+  intros x hx h_eqone.
+  (* specevar h_eqone at y. *)
+  especialize h_eqone using (! ! ! # ! ! ##).
+  + subst.
+    Fail
+      (* this should fail if there are only nat hyps: *)
+      ltac:(match goal with
+            | H: ?t |- a = 1 =>
+                match t with
+                  nat => fail 1
+                | _ => idtac "remaining hyp: " H ":" t 
+                end
+            end).
+Abort.
+
+
+End At.
