LibHyps/LibSpecialize.v
@@ -2,6 +2,46 @@
   This file is part of LibHyps. It is distributed under the MIT
   "expat license". You should have recieved a LICENSE file with it. *)
 
+(* The especialize tactic allows to create subgoals from premises of a
+   hypothesis.
+
+From a hypothesis of the form:
+
+H: forall a b c, A -> B -> C -> X
+
+one can start a goal for either A and/or B and/or C, while making
+evars for a and/pr b and/or c. Duplicating H or not.
+
+especialize H with a at 2.
+
+will start a goal GB of type B[a<-?a] and specialize H with ?a and GB.
+Changing H into:
+
+H: forall b c, A[a<-?a] -> C[a<-?a} -> X[a<-?a]
+
+Note that B must be proved without without supposing A. This tactic
+does not implement the exact logical rule (this is work in progress).
+This limitation is however not a problem in practice: if B needs A
+then the user almost always wants to prove A first.
+
+The tactic supports sevral evars and/or several sibgoals at once:
+
+especialize H with a,b at 1,2.
+etc.
+
+Special "at *" form (inspired by exploit from Compcert=::
+
+especialize H with a,b,c at *.
+
+will start goals for all premises (A, B and C in the example above).
+
+Special "until" form e.g. :
+
+especialize with a,c A until 2.
+
+will start goals for all the 2 first premises  with evars ?a, and ?c. *)
+
+
 (* proveprem H at i as h. Create an assert for the ith dependent
 premiss of hypothesis H and specialize H with the resulting proof. h
 is the (optional) name of the asserted premiss. *)
@@ -16,6 +56,12 @@ Ltac fresh_unfail H :=
     | _ => fresh "H_"
   end.
 
+Ltac fail_if_not_hyp c :=
+  (is_var(c))
+  + ((assert_fails (is_var(c)));
+     fail "especialize: please provide a name for the new hyp (with 'as')").
+
+
 Ltac proveprem_as_prem H i idpremis idnewH :=
   (* prefer this to evar, which is not well "typed" by Ltac (does not
      know that it creates an evar (coq bug?). *)
@@ -23,24 +69,21 @@ Ltac proveprem_as_prem H i idpremis idnewH :=
   assert (idpremis:ev);
   [|specialize H with (i:=idpremis) as idnewH].
 
-Tactic Notation "especialize" constr(H) "at" integer(i) "as" ident(idH) ":" ident(idprem) := proveprem_as_prem H i idprem idH.
-Tactic Notation "especialize" constr(H) "as" ident(idH) "at" integer(i) ":" ident(idprem) := proveprem_as_prem H i idprem idH.
+Tactic Notation "especialize" constr(H) "at" int_or_var(i) "as" ident(idH) ":" ident(idprem) := proveprem_as_prem H i idprem idH.
 
 Ltac proveprem_asg_newH H i idpremis :=
   let prefx := fresh_unfail H in
   let idnewH := fresh prefx "spec" in (* FIXME: if H is not freshable? *)
   proveprem_as_prem H i idpremis idnewH.
 
-Tactic Notation "especialize" constr(H) "at" integer(i) "as" "?" ":" ident(idprem) := proveprem_asg_newH H i idprem.
-Tactic Notation "especialize" constr(H) "as" "?" "at" integer(i) ":" ident(idprem) := proveprem_asg_newH H i idprem.
+Tactic Notation "especialize" constr(H) "at" int_or_var(i) "as" "?" ":" ident(idprem) := proveprem_asg_newH H i idprem.
 
 Ltac proveprem_as_premg H i idnewH :=
   let prefx := fresh_unfail H in
   let idpremis := fresh prefx "prem" in
   proveprem_as_prem H i idpremis idnewH.
 
-Tactic Notation "especialize" constr(H) "at" integer(i) "as" ident(idH) ":" "?" := proveprem_as_premg H i idH.
-Tactic Notation "especialize" constr(H) "as" ident(idH) "at" integer(i) ":" "?" := proveprem_as_premg H i idH.
+Tactic Notation "especialize" constr(H) "at" int_or_var(i) "as" ident(idH) ":" "?" := proveprem_as_premg H i idH.
 
 
 Ltac proveprem_asg_premg H i :=
@@ -49,16 +92,14 @@ Ltac proveprem_asg_premg H i :=
   let idpremis := fresh prefx "prem" in
   proveprem_as_prem H i idpremis idnewH.
 
-Tactic Notation "especialize" constr(H) "at" integer(i) "as" "?" ":" "?" := proveprem_asg_premg H i.
-Tactic Notation "especialize" constr(H) "as" "?" "at" integer(i) ":" "?" := proveprem_asg_premg H i.
+Tactic Notation "especialize" constr(H) "at" int_or_var(i) "as" "?" ":" "?" := proveprem_asg_premg H i.
 
 Ltac proveprem_as H i idnewH :=
   let prefx := fresh_unfail H in
   let idpremis := fresh prefx "prem" in
   proveprem_as_prem H i idpremis idnewH;[ | clear idpremis].
 
-Tactic Notation "especialize" constr(H) "at" integer(i) "as" ident(idH) := proveprem_as H i idH.
-Tactic Notation "especialize" constr(H) "as" ident(idH) "at" integer(i) := proveprem_as H i idH.
+Tactic Notation "especialize" constr(H) "at" int_or_var(i) "as" ident(idH) := proveprem_as H i idH.
 
 
 Ltac proveprem_asg H i :=
@@ -67,9 +108,7 @@ Ltac proveprem_asg H i :=
   let idpremis := fresh prefx "prem" in
   proveprem_as_prem H i idpremis idnewH;[ | clear idpremis].
 
-Tactic Notation "especialize" constr(H) "at" integer(i) "as" "?" := proveprem_asg H i.
-Tactic Notation "especialize" constr(H) "as" "?" "at" integer(i) := proveprem_asg H i.
-
+Tactic Notation "especialize" constr(H) "at" int_or_var(i) "as" "?" := proveprem_asg H i.
 
 
 (* Version where specialize is not given a name (soeither H is a
@@ -80,14 +119,16 @@ Ltac proveprem_prem H i idpremis :=
   assert (idpremis:ev);
   [|specialize H with (i:=idpremis)].
 
-Tactic Notation "especialize" constr(H) "at" integer(i) ":" ident(idprem) := proveprem_prem H i idprem.
+Tactic Notation "especialize" constr(H) "at" int_or_var(i) ":" ident(idprem) :=
+  fail_if_not_hyp H;
+  proveprem_prem H i idprem.
 
 Ltac proveprem_premg H i :=
   let prefx := fresh_unfail H in
   let idpremis := fresh prefx "prem" in
   proveprem_prem H i idpremis.
 
-Tactic Notation "especialize" constr(H) "at" integer(i) ":" "?" := proveprem_premg H i.
+Tactic Notation "especialize" constr(H) "at" int_or_var(i) ":" "?" := proveprem_premg H i.
 
 (* same as proveprem_prem but discard the created hypothesis once used in specialization *)
 Ltac proveprem H i :=
@@ -95,13 +136,12 @@ Ltac proveprem H i :=
   let idpremis := fresh prefx "prem" in
   proveprem_prem H i idpremis ; [ | clear idpremis].
 
-Tactic Notation "especialize" constr(H) "at" integer(i) := proveprem H i.
-Tactic Notation "especialize" constr(H) "at" integer(i) := proveprem H i.
-
+Tactic Notation "especialize" constr(H) "at" int_or_var(i) := fail_if_not_hyp H;proveprem H i.
 
 (* Create a subgoal for each dependent premiss of H *)
 Ltac proveprem_all H := (especialize H at 1; [| proveprem_all H]) + idtac.
 
+(* TODO: make the "as" mandatory if G not a hyp. *)
 Tactic Notation "especialize" constr(H) "at" "*" :=
   ((try (is_var(H); fail 1));
    (let prefx := fresh_unfail H in
@@ -122,6 +162,7 @@ Ltac proveprem_until H i :=
   | (S ?i') => (especialize H at 1; [| proveprem_until H i'])
   end.
 
+(* TODO idem: make as mandatory *)
 Tactic Notation "especialize" constr(H) "until" constr(i) :=
   (try (is_var(H); fail 1);
    (let prefx := fresh_unfail H in
@@ -147,8 +188,7 @@ Ltac proveprem_as_2 H idnewH i1 i2 :=
     assert (idprem2:ev2);
     [|specialize H with (i1:=idprem1) (i2:=idprem2) as idnewH ; clear idprem2 idprem1]].
 
-Tactic Notation "especialize" constr(H) "as" ident(idH) "at"  integer(i1) "," integer(i2) := proveprem_as_2 H idH i1 i2.
-Tactic Notation "especialize" constr(H) "at"  integer(i1) "," integer(i2) "as" ident(idH) := proveprem_as_2 H idH i1 i2.
+Tactic Notation "especialize" constr(H) "at"  int_or_var(i1) "," int_or_var(i2) "as" ident(idH) := proveprem_as_2 H idH i1 i2.
 
 (* Same but discard the created hypothesis once used in specialization *)
 Ltac proveprem_2 H i1 i2 :=
@@ -162,7 +202,7 @@ Ltac proveprem_2 H i1 i2 :=
     assert (idprem2:ev2);
     [|specialize H with (i1:=idprem1) (i2:=idprem2) ; clear idprem2 idprem1]].
 
-Tactic Notation "especialize" constr(H) "at" integer(i1) "," integer(i2) := proveprem_2 H i1 i2.
+Tactic Notation "especialize" constr(H) "at" int_or_var(i1) "," int_or_var(i2) := proveprem_2 H i1 i2.
 
 Ltac proveprem_as_3 H idnewH i1 i2 i3 :=
   let prefx := fresh_unfail H in
@@ -177,8 +217,7 @@ Ltac proveprem_as_3 H idnewH i1 i2 i3 :=
       [ | assert (idprem3:ev3);
           [ | specialize H with (i1:=idprem1) (i2:=idprem2) (i3:=idprem3) as idnewH ; clear idprem3 idprem2 idprem1 ]]].
 
-Tactic Notation "especialize" constr(H) "as" ident(idH) "at"  integer(i1) "," integer(i2)"," integer(i3) := proveprem_as_3 H idH i1 i2 i3.
-Tactic Notation "especialize" constr(H) "at"  integer(i1) "," integer(i2)"," integer(i3) "as" ident(idH) := proveprem_as_3 H idH i1 i2 i3.
+Tactic Notation "especialize" constr(H) "at"  int_or_var(i1) "," int_or_var(i2)"," int_or_var(i3) "as" ident(idH) := proveprem_as_3 H idH i1 i2 i3.
 
 Ltac proveprem_3 H i1 i2 i3 :=
   let prefx := fresh_unfail H in
@@ -193,7 +232,7 @@ Ltac proveprem_3 H i1 i2 i3 :=
       [ | assert (idprem3:ev3);
           [ | specialize H with (i1:=idprem1) (i2:=idprem2) (i3:=idprem3) ; clear idprem3 idprem2 idprem1 ]]].
 
-Tactic Notation "especialize" constr(H) "at"  integer(i1) "," integer(i2)"," integer(i3) := proveprem_3 H i1 i2 i3.
+Tactic Notation "especialize" constr(H) "at"  int_or_var(i1) "," int_or_var(i2)"," int_or_var(i3) := proveprem_3 H i1 i2 i3.
 
 Ltac proveprem_as_4 H idnewH i1 i2 i3 i4 :=
   let prefx := fresh_unfail H in
@@ -212,8 +251,7 @@ Ltac proveprem_as_4 H idnewH i1 i2 i3 i4 :=
         [ | specialize H with (i1:=idprem1) (i2:=idprem2) (i3:=idprem3) (i4:=idprem4) as idnewH ;
             clear idprem4 idprem3 idprem2 idprem1 ]]]].
 
-Tactic Notation "especialize" constr(H) "as" ident(idH) "at"  integer(i1) "," integer(i2) "," integer(i3) "," integer(i4) := proveprem_as_4 H idH i1 i2 i3 i4.
-Tactic Notation "especialize" constr(H) "at"  integer(i1) "," integer(i2)"," integer(i3) "," integer(i4) "as" ident(idH) := proveprem_as_4 H idH i1 i2 i3 i4.
+Tactic Notation "especialize" constr(H) "at"  int_or_var(i1) "," int_or_var(i2)"," int_or_var(i3) "," int_or_var(i4) "as" ident(idH) := proveprem_as_4 H idH i1 i2 i3 i4.
 
 Ltac proveprem_4 H i1 i2 i3 i4 :=
   let prefx := fresh_unfail H in
@@ -232,7 +270,7 @@ Ltac proveprem_4 H i1 i2 i3 i4 :=
         [ | specialize H with (i1:=idprem1) (i2:=idprem2) (i3:=idprem3) (i4:=idprem4) ;
             clear idprem4 idprem3 idprem2 idprem1 ]]]].
 
-Tactic Notation "especialize" constr(H) "at"  integer(i1) "," integer(i2)"," integer(i3) "," integer(i4) := proveprem_4 H i1 i2 i3 i4.
+Tactic Notation "especialize" constr(H) "at"  int_or_var(i1) "," int_or_var(i2)"," int_or_var(i3) "," int_or_var(i4) := proveprem_4 H i1 i2 i3 i4.
 
 
 Ltac proveprem_as_5 H idnewH i1 i2 i3 i4 i5 :=
@@ -255,8 +293,7 @@ Ltac proveprem_as_5 H idnewH i1 i2 i3 i4 i5 :=
           | specialize H with (i1:=idprem1) (i2:=idprem2) (i3:=idprem3) (i4:=idprem4) (i5:=idprem5) as idnewH ;
             clear idprem5 idprem4 idprem3 idprem2 idprem1 ]]]]].
 
-Tactic Notation "especialize" constr(H) "as" ident(idH) "at"  integer(i1) "," integer(i2) "," integer(i3) "," integer(i4) "," integer(i5) := proveprem_as_5 H idH i1 i2 i3 i4 i5.
-Tactic Notation "especialize" constr(H) "at"  integer(i1) "," integer(i2)"," integer(i3) "," integer(i4) "," integer(i5) "as" ident(idH) := proveprem_as_5 H idH i1 i2 i3 i4 i5.
+Tactic Notation "especialize" constr(H) "at"  int_or_var(i1) "," int_or_var(i2)"," int_or_var(i3) "," int_or_var(i4) "," int_or_var(i5) "as" ident(idH) := proveprem_as_5 H idH i1 i2 i3 i4 i5.
 
 Ltac proveprem_5 H i1 i2 i3 i4 i5 :=
   let prefx := fresh_unfail H in
@@ -278,7 +315,7 @@ Ltac proveprem_5 H i1 i2 i3 i4 i5 :=
           | specialize H with (i1:=idprem1) (i2:=idprem2) (i3:=idprem3) (i4:=idprem4) (i5:=idprem5);
             clear idprem5 idprem4 idprem3 idprem2 idprem1 ]]]]].
 
-Tactic Notation "especialize" constr(H) "at"  integer(i1) "," integer(i2)"," integer(i3) "," integer(i4) "," integer(i5) := proveprem_5 H i1 i2 i3 i4 i5.
+Tactic Notation "especialize" constr(H) "at"  int_or_var(i1) "," int_or_var(i2)"," int_or_var(i3) "," int_or_var(i4) "," int_or_var(i5) := proveprem_5 H i1 i2 i3 i4 i5.
 
 Ltac proveprem_as_6 H idnewH i1 i2 i3 i4 i5 i6 :=
   let prefx := fresh_unfail H in
@@ -303,8 +340,7 @@ Ltac proveprem_as_6 H idnewH i1 i2 i3 i4 i5 i6 :=
             | specialize H with (i1:=idprem1) (i2:=idprem2) (i3:=idprem3) (i4:=idprem4) (i5:=idprem5) (i6:=idprem6) as idnewH ;
               clear idprem6 idprem5 idprem4 idprem3 idprem2 idprem1 ]]]]]].
 
-Tactic Notation "especialize" constr(H) "as" ident(idH) "at"  integer(i1) "," integer(i2) "," integer(i3) "," integer(i4) "," integer(i5) "," integer(i6) := proveprem_as_6 H idH i1 i2 i3 i4 i5 i6.
-Tactic Notation "especialize" constr(H) "at"  integer(i1) "," integer(i2)"," integer(i3) "," integer(i4) "," integer(i5) "," integer(i6) "as" ident(idH) := proveprem_as_6 H idH i1 i2 i3 i4 i5 i6.
+Tactic Notation "especialize" constr(H) "at"  int_or_var(i1) "," int_or_var(i2)"," int_or_var(i3) "," int_or_var(i4) "," int_or_var(i5) "," int_or_var(i6) "as" ident(idH) := proveprem_as_6 H idH i1 i2 i3 i4 i5 i6.
 
 Ltac proveprem_6 H i1 i2 i3 i4 i5 i6 :=
   let prefx := fresh_unfail H in
@@ -329,7 +365,7 @@ Ltac proveprem_6 H i1 i2 i3 i4 i5 i6 :=
           | specialize H with (i1:=idprem1) (i2:=idprem2) (i3:=idprem3) (i4:=idprem4) (i5:=idprem5) (i6:=idprem6);
             clear idprem6 idprem5 idprem4 idprem3 idprem2 idprem1 ]]]]]].
 
-Tactic Notation "especialize" constr(H) "at"  integer(i1) "," integer(i2)"," integer(i3) "," integer(i4) "," integer(i5) "," integer(i6) := proveprem_6 H i1 i2 i3 i4 i5 i6.
+Tactic Notation "especialize" constr(H) "at"  int_or_var(i1) "," int_or_var(i2)"," int_or_var(i3) "," int_or_var(i4) "," int_or_var(i5) "," int_or_var(i6) := proveprem_6 H i1 i2 i3 i4 i5 i6.
 
 Ltac proveprem_as_7 H idnewH i1 i2 i3 i4 i5 i6 i7 :=
   let prefx := fresh_unfail H in
@@ -357,8 +393,7 @@ Ltac proveprem_as_7 H idnewH i1 i2 i3 i4 i5 i6 i7 :=
               | specialize H with (i1:=idprem1) (i2:=idprem2) (i3:=idprem3) (i4:=idprem4) (i5:=idprem5) (i6:=idprem6) (i7:=idprem7) as idnewH ;
                 clear idprem7 idprem6 idprem5 idprem4 idprem3 idprem2 idprem1 ]]]]]]].
 
-Tactic Notation "especialize" constr(H) "as" ident(idH) "at"  integer(i1) "," integer(i2) "," integer(i3) "," integer(i4) "," integer(i5) "," integer(i6) "," integer(i7) := proveprem_as_7 H idH i1 i2 i3 i4 i5 i6 i7.
-Tactic Notation "especialize" constr(H) "at"  integer(i1) "," integer(i2)"," integer(i3) "," integer(i4) "," integer(i5) "," integer(i6) "," integer(i7) "as" ident(idH) := proveprem_as_7 H idH i1 i2 i3 i4 i5 i6 i7.
+Tactic Notation "especialize" constr(H) "at"  int_or_var(i1) "," int_or_var(i2)"," int_or_var(i3) "," int_or_var(i4) "," int_or_var(i5) "," int_or_var(i6) "," int_or_var(i7) "as" ident(idH) := proveprem_as_7 H idH i1 i2 i3 i4 i5 i6 i7.
 
 Ltac proveprem_7 H i1 i2 i3 i4 i5 i6 i7:=
   let prefx := fresh_unfail H in
@@ -386,52 +421,625 @@ Ltac proveprem_7 H i1 i2 i3 i4 i5 i6 i7:=
               | specialize H with (i1:=idprem1) (i2:=idprem2) (i3:=idprem3) (i4:=idprem4) (i5:=idprem5) (i6:=idprem6) (i7:=idprem7);
                 clear idprem7 idprem6 idprem5 idprem4 idprem3 idprem2 idprem1 ]]]]]]].
 
-Tactic Notation "especialize" constr(H) "at"  integer(i1) "," integer(i2)"," integer(i3) "," integer(i4) "," integer(i5) "," integer(i6) "," integer(i7) := proveprem_7 H i1 i2 i3 i4 i5 i6 i7.
+Tactic Notation "especialize" constr(H) "at"  int_or_var(i1) "," int_or_var(i2)"," int_or_var(i3) "," int_or_var(i4) "," int_or_var(i5) "," int_or_var(i6) "," int_or_var(i7) := proveprem_7 H i1 i2 i3 i4 i5 i6 i7.
+
+
+Tactic Notation "especialize" constr(H) "at" int_or_var(i) "as" "?" :=
+  let nme := fresh in
+  especialize H at i as nme.
+
+Tactic Notation "especialize" constr(H) "at" int_or_var(i1) "," int_or_var(i2) "as" "?" :=
+  let nme := fresh in
+  especialize H at i1,i2 as nme.
+
+Tactic Notation "especialize" constr(H) "at" int_or_var(i1) "," int_or_var(i2)  "," int_or_var(i3) "as" "?" :=
+  let nme := fresh in
+  especialize H at i1,i2,i3 as nme.
+
+Tactic Notation "especialize" constr(H) "at" int_or_var(i1) "," int_or_var(i2)  "," int_or_var(i3) "," int_or_var(i4) "as" "?" :=
+  let nme := fresh in
+  especialize H at i1,i2,i3,i4 as nme.
+
+Tactic Notation "especialize" constr(H) "at" int_or_var(i1) "," int_or_var(i2) "," int_or_var(i3) "," int_or_var(i4) "," int_or_var(i5) "as" "?" :=
+  let nme := fresh in
+  especialize H at i1,i2,i3,i4,i5 as nme.
+
+Tactic Notation "especialize" constr(H) "at" int_or_var(i1) "," int_or_var(i2) "," int_or_var(i3) "," int_or_var(i4) "," int_or_var(i5) "," int_or_var(i6) "as" "?" :=
+  let nme := fresh in
+  especialize H at i1,i2,i3,i4,i5,i6 as nme.
+
+Tactic Notation "especialize" constr(H) "at" int_or_var(i1) "," int_or_var(i2) "," int_or_var(i3) "," int_or_var(i4) "," int_or_var(i5) "," int_or_var(i6) "," int_or_var(i7) "as" "?" :=
+  let nme := fresh in
+  especialize H at i1,i2,i3,i4,i5,i6,i7 as nme.
 
 
 
-(*
-Definition eq_one (i:nat) := i = 1.
 
-Lemma test_esepec_6_7: (eq_one 2 -> eq_one 3 ->eq_one 4 ->eq_one 5 ->eq_one 6 ->eq_one 7 ->eq_one 8 -> eq_one 9 -> eq_one 1 -> False) -> True.
-Proof.
-  intros H.
-  especialize H at 3,1,4,5,2,7 as h; [ admit | admit | admit  | admit | admit | admit | match type of h with eq_one 7 -> eq_one 9 -> eq_one 1 ->False=> idtac "OK" end].
-  Undo.
-  especialize H as h at 3,1,4,5,2,7; [ admit | admit | admit  | admit | admit | admit | match type of h with eq_one 7 -> eq_one 9 -> eq_one 1 ->False=> idtac "OK" end].
-  Undo.
-  especialize H at 3,1,4,5,2,7; [ admit | admit | admit  | admit | admit | admit | match type of H with eq_one 7 -> eq_one 9 -> eq_one 1 ->False=> idtac "OK" end].
-  Undo.
-  especialize H at 3,1,4,5,2,7,9 as h; [ admit | admit | admit  | admit | admit | admit | admit | match type of h with eq_one 7 -> eq_one 9 -> False => idtac "OK" end].
-  Undo.
-  especialize H as h at 3,1,4,5,2,7,9; [ admit | admit | admit  | admit | admit | admit | admit | match type of h with eq_one 7 -> eq_one 9 -> False => idtac "OK" end].
-  Undo.
-  especialize H at 3,1,4,5,2,7,9; [ admit | admit | admit  | admit | admit | admit | admit | match type of H with eq_one 7 -> eq_one 9 -> False => idtac "OK" end].
-  Undo.
-  exact I.
-Qed.
+(* Adding a phase of evar creation for premises that should be solved
+   by side effect of proving others. NOTE that there is no mechanism
+   to ensure that these evar are actually solved when subgoals are
+   proved. You may want to try "unshelve especialize ..." to have a
+   look at created evars.
+
+NOTE: All these tactic notations would be greatly simplified if there
+were a way of iterating on a list_int_sep and/or on list_ident_sep and
+on the list of "with bindindgs". Probablt Ltac2 would be much better
+at this. *)
+
+Ltac spec_evar H id_name :=
+  let idt := fresh id_name "T" in
+  let id := fresh id_name in
+  evar (idt : Type);
+  evar (id : idt);
+  specialize H with (id_name := id); subst id; subst idt.
 
 
+Tactic Notation "especialize" constr(H) "with" ident(id) "at" "*" :=
+  fail_if_not_hyp H;
+  spec_evar H id;
+  especialize H at * .
+Tactic Notation "especialize" constr(oldH) "with" ident(id) "at" "*" "as" ident(H) :=
+  specialize oldH as H;
+  especialize H with id at *.
+Tactic Notation "especialize" constr(H) "with" ident(id) "at" "*" "as" "?" :=
+  let nme := fresh in
+  especialize H with id at * as nme.
+
+Tactic Notation "especialize" constr(H) "with" ident(id) "until" constr(i) :=
+  fail_if_not_hyp H;
+  spec_evar H id;
+  especialize H until i .
+Tactic Notation "especialize" constr(oldH) "with" ident(id) "until" constr(i) "as" ident(H) :=
+  specialize oldH as H;
+  especialize H with id until i.
+Tactic Notation "especialize" constr(H) "with" ident(id) "until" constr(i) "as" "?" :=
+  let nme := fresh in
+  especialize H with id until i as nme.
+
+Tactic Notation "especialize" constr(H) "with" ident(id) "at" int_or_var(i) :=
+  fail_if_not_hyp H;
+  spec_evar H id;
+  especialize H at i .
+Tactic Notation "especialize" constr(oldH) "with" ident(id) "at" int_or_var(i) "as" ident(H) :=
+  specialize oldH as H;
+  especialize H with id at i.
+Tactic Notation "especialize" constr(H) "with" ident(id) "at" int_or_var(i) "as" "?" :=
+  let nme := fresh in
+  especialize H with id at i as nme.
+
+Tactic Notation "especialize" constr(H) "with" ident(id) "at" int_or_var(i) ":" ident(hprem) :=
+  fail_if_not_hyp H;
+  spec_evar H id;
+  especialize H at i : hprem.
+Tactic Notation "especialize" constr(oldH) "with" ident(id) "at" int_or_var(i) "as" ident(H) ":"  ident(hprem) :=
+  specialize oldH as H;
+  especialize H with id at i : hprem.
+Tactic Notation "especialize" constr(H) "with" ident(id) "at" int_or_var(i) "as" "?" ":"  ident(hprem) :=
+  let nme := fresh in
+  especialize H with id at i as nme : hprem.
+
+Tactic Notation "especialize" constr(H) "with" ident(id) "at" int_or_var(i1) "," int_or_var(i2) :=
+  fail_if_not_hyp H;
+  spec_evar H id;
+  especialize H at i1,i2 .
+Tactic Notation "especialize" constr(oldH) "with" ident(id) "at" int_or_var(i1) "," int_or_var(i2) "as" ident(H) :=
+  specialize oldH as H;
+  especialize H with id at i1,i2.
+Tactic Notation "especialize" constr(H) "with" ident(id) "at" int_or_var(i1) "," int_or_var(i2) "as" "?" :=
+  let nme := fresh in
+  especialize H with id at i1,i2 as nme.
+
+Tactic Notation "especialize" constr(H) "with" ident(id) "at" int_or_var(i1) "," int_or_var(i2)  "," int_or_var(i3) :=
+  fail_if_not_hyp H;
+  spec_evar H id;
+  especialize H at i1,i2,i3.
+Tactic Notation "especialize" constr(oldH) "with" ident(id) "at" int_or_var(i1) "," int_or_var(i2)  "," int_or_var(i3) "as" ident(H) :=
+  specialize oldH as H;
+  especialize H with id at i1,i2,i3.
+Tactic Notation "especialize" constr(H) "with" ident(id) "at" int_or_var(i1) "," int_or_var(i2)  "," int_or_var(i3) "as" "?" :=
+  let nme := fresh in
+  especialize H with id at i1,i2,i3 as nme.
+
+Tactic Notation "especialize" constr(H) "with" ident(id) "at" int_or_var(i1) "," int_or_var(i2)  "," int_or_var(i3) "," int_or_var(i4) :=
+  fail_if_not_hyp H;
+  spec_evar H id;
+  especialize H at i1,i2,i3,i4 .
+Tactic Notation "especialize" constr(oldH) "with" ident(id) "at" int_or_var(i1) "," int_or_var(i2)  "," int_or_var(i3) "," int_or_var(i4) "as" ident(H) :=
+  specialize oldH as H;
+  especialize H with id at i1,i2,i3,i4.
+Tactic Notation "especialize" constr(H) "with" ident(id) "at" int_or_var(i1) "," int_or_var(i2)  "," int_or_var(i3) "," int_or_var(i4) "as" "?" :=
+  let nme := fresh in
+  especialize H with id at i1,i2,i3,i4 as nme.
+
+Tactic Notation "especialize" constr(H) "with" ident(id) "at" int_or_var(i1) "," int_or_var(i2) "," int_or_var(i3) "," int_or_var(i4) "," int_or_var(i5) :=
+  fail_if_not_hyp H;
+  spec_evar H id;
+  especialize H at i1,i2,i3,i4,i5 .
+Tactic Notation "especialize" constr(oldH) "with" ident(id) "at" int_or_var(i1) "," int_or_var(i2) "," int_or_var(i3) "," int_or_var(i4) "," int_or_var(i5) "as" ident(H) :=
+  specialize oldH as H;
+  especialize H with id at i1,i2,i3,i4,i5 .
+Tactic Notation "especialize" constr(H) "with" ident(id) "at" int_or_var(i1) "," int_or_var(i2) "," int_or_var(i3) "," int_or_var(i4) "," int_or_var(i5) "as" "?" :=
+  let nme := fresh in
+  especialize H with id at i1,i2,i3,i4,i5 as nme.
+
+Tactic Notation "especialize" constr(H) "with" ident(id) "at" int_or_var(i1) "," int_or_var(i2) "," int_or_var(i3) "," int_or_var(i4) "," int_or_var(i5) "," int_or_var(i6) :=
+  fail_if_not_hyp H;
+  spec_evar H id;
+  especialize H at i1,i2,i3,i4,i5,i6.
+Tactic Notation "especialize" constr(oldH) "with" ident(id) "at" int_or_var(i1) "," int_or_var(i2) "," int_or_var(i3) "," int_or_var(i4) "," int_or_var(i5) "," int_or_var(i6) "as" ident(H) :=
+  specialize oldH as H;
+  especialize H with id at i1,i2,i3,i4,i5,i6.
+Tactic Notation "especialize" constr(H) "with" ident(id) "at" int_or_var(i1) "," int_or_var(i2) "," int_or_var(i3) "," int_or_var(i4) "," int_or_var(i5) "," int_or_var(i6) "as" "?" :=
+  let nme := fresh in
+  especialize H with id at i1,i2,i3,i4,i5,i6 as nme.
+
+Tactic Notation "especialize" constr(H) "with" ident(id) "at" int_or_var(i1) "," int_or_var(i2) "," int_or_var(i3) "," int_or_var(i4) "," int_or_var(i5) "," int_or_var(i6) "," int_or_var(i7) :=
+  fail_if_not_hyp H;
+  spec_evar H id;
+  especialize H at i1,i2,i3,i4,i5,i6,i7.
+Tactic Notation "especialize" constr(oldH) "with" ident(id) "at" int_or_var(i1) "," int_or_var(i2) "," int_or_var(i3) "," int_or_var(i4) "," int_or_var(i5) "," int_or_var(i6) "," int_or_var(i7) "as" ident(H) :=
+  specialize oldH as H;
+  especialize H with id at i1,i2,i3,i4,i5,i6,i7.
+Tactic Notation "especialize" constr(H) "with" ident(id) "at" int_or_var(i1) "," int_or_var(i2) "," int_or_var(i3) "," int_or_var(i4) "," int_or_var(i5) "," int_or_var(i6) "," int_or_var(i7) "as" "?" :=
+  let nme := fresh in
+  especialize H with id at i1,i2,i3,i4,i5,i6,i7 as nme.
+
+
+Tactic Notation "especialize" constr(H) "with" ident(id1) "," ident(id2) "at" "*" :=
+  fail_if_not_hyp H;
+  spec_evar H id1;
+  especialize H with id2 at *.
+Tactic Notation "especialize" constr(oldH) "with" ident(id1) "," ident(id2) "at" "*" "as" ident(H) :=
+  specialize oldH as H;
+  especialize H with id1,id2 at *.
+Tactic Notation "especialize" constr(H) "with" ident(id1) "," ident(id2) "at" "*" "as" "?" :=
+  let nme := fresh in
+  especialize H with id1,id2 at * as nme.
+
+Tactic Notation "especialize" constr(H) "with" ident(id1) "," ident(id2) "until" constr(i) :=
+  fail_if_not_hyp H;
+  spec_evar H id1;
+  especialize H with id2 until i .
+Tactic Notation "especialize" constr(oldH) "with" ident(id1) "," ident(id2) "until" constr(i) "as" ident(H) :=
+  specialize oldH as H;
+  especialize H with id1,id2 until i .
+Tactic Notation "especialize" constr(H) "with" ident(id1) "," ident(id2) "until" constr(i) "as" "?" :=
+  let nme := fresh in
+  especialize H with id1,id2 until i as nme.
+
+Tactic Notation "especialize" constr(H) "with" ident(id1) "," ident(id2) "at" int_or_var(i) :=
+  fail_if_not_hyp H;
+  spec_evar H id1;
+  especialize H with id2 at i .
+Tactic Notation "especialize" constr(oldH) "with" ident(id1) "," ident(id2) "at" int_or_var(i) "as" ident(H) :=
+  specialize oldH as H;
+  especialize H with id1,id2 at i .
+Tactic Notation "especialize" constr(H) "with" ident(id1) "," ident(id2) "at" int_or_var(i) "as" "?" :=
+  let nme := fresh in
+  especialize H with id1,id2 at i as nme.
+
+Tactic Notation "especialize" constr(H) "with" ident(id1) "," ident(id2) "at" int_or_var(i) ":" ident(hprem) :=
+  fail_if_not_hyp H;
+  spec_evar H id1;
+  especialize H with id2 at i : hprem.
+Tactic Notation "especialize" constr(oldH) "with" ident(id1) "," ident(id2) "at" int_or_var(i) "as" ident(H) ":" ident(hprem) :=
+  specialize oldH as H;
+  especialize H with id1,id2 at i : hprem.
+Tactic Notation "especialize" constr(H) "with" ident(id1) "," ident(id2) "at" int_or_var(i) "as" "?" ":" ident(hprem) :=
+  let nme := fresh in
+  especialize H with id1,id2 at i as nme : hprem.
+
+Tactic Notation "especialize" constr(H) "with" ident(id1) "," ident(id2) "at" int_or_var(i1) "," int_or_var(i2) :=
+  fail_if_not_hyp H;
+  spec_evar H id1;
+  especialize H with id2 at i1,i2 .
+Tactic Notation "especialize" constr(oldH) "with" ident(id1) "," ident(id2) "at" int_or_var(i1) "," int_or_var(i2) "as" ident(H) :=
+  specialize oldH as H;
+  especialize H with id1,id2 at i1,i2 .
+Tactic Notation "especialize" constr(H) "with" ident(id1) "," ident(id2) "at" int_or_var(i1) "," int_or_var(i2) "as" "?" :=
+  let nme := fresh in
+  especialize H with id1,id2 at i1,i2 as nme.
+
+Tactic Notation "especialize" constr(H) "with" ident(id1) "," ident(id2) "at" int_or_var(i1) "," int_or_var(i2) "," int_or_var(i3) :=
+  fail_if_not_hyp H;
+  spec_evar H id1;
+  especialize H with id2 at i1,i2,i3 .
+Tactic Notation "especialize" constr(oldH) "with" ident(id1) "," ident(id2) "at" int_or_var(i1) "," int_or_var(i2) "," int_or_var(i3) "as" ident(H) :=
+  specialize oldH as H;
+  especialize H with id1,id2 at i1,i2,i3 .
+Tactic Notation "especialize" constr(H) "with" ident(id1) "," ident(id2) "at" int_or_var(i1) "," int_or_var(i2) "," int_or_var(i3) "as" "?" :=
+  let nme := fresh in
+  especialize H with id1,id2 at i1,i2,i3 as nme.
+
+Tactic Notation "especialize" constr(H) "with" ident(id1) "," ident(id2) "at" int_or_var(i1) "," int_or_var(i2)  "," int_or_var(i3) "," int_or_var(i4) :=
+  fail_if_not_hyp H;
+  spec_evar H id1;
+  especialize H with id2 at i1,i2,i3,i4 .
+Tactic Notation "especialize" constr(oldH) "with" ident(id1) "," ident(id2) "at" int_or_var(i1) "," int_or_var(i2)  "," int_or_var(i3) "," int_or_var(i4) "as" ident(H) :=
+  specialize oldH as H;
+  especialize H with id1,id2 at i1,i2,i3,i4 .
+Tactic Notation "especialize" constr(H) "with" ident(id1) "," ident(id2) "at" int_or_var(i1) "," int_or_var(i2)  "," int_or_var(i3) "," int_or_var(i4) "as" "?" :=
+  let nme := fresh in
+  especialize H with id1,id2 at i1,i2,i3,i4 as nme.
+
+Tactic Notation "especialize" constr(H) "with" ident(id1) "," ident(id2) "at" int_or_var(i1) "," int_or_var(i2) "," int_or_var(i3) "," int_or_var(i4) "," int_or_var(i5) :=
+  fail_if_not_hyp H;
+  spec_evar H id1;
+  especialize H with id2 at i1,i2,i3,i4,i5 .
+Tactic Notation "especialize" constr(oldH) "with" ident(id1) "," ident(id2) "at" int_or_var(i1) "," int_or_var(i2) "," int_or_var(i3) "," int_or_var(i4) "," int_or_var(i5) "as" ident(H) :=
+  specialize oldH as H;
+  especialize H with id1,id2 at i1,i2,i3,i4,i5 .
+Tactic Notation "especialize" constr(H) "with" ident(id1) "," ident(id2) "at" int_or_var(i1) "," int_or_var(i2) "," int_or_var(i3) "," int_or_var(i4) "," int_or_var(i5) "as" "?" :=
+  let nme := fresh in
+  especialize H with id1,id2 at i1,i2,i3,i4,i5 as nme.
+
+Tactic Notation "especialize" constr(H) "with" ident(id1) "," ident(id2) "at" int_or_var(i1) "," int_or_var(i2) "," int_or_var(i3) "," int_or_var(i4) "," int_or_var(i5) "," int_or_var(i6) :=
+  fail_if_not_hyp H;
+  spec_evar H id1;
+  especialize H with id2 at i1,i2,i3,i4,i5,i6 .
+Tactic Notation "especialize" constr(oldH) "with" ident(id1) "," ident(id2) "at" int_or_var(i1) "," int_or_var(i2) "," int_or_var(i3) "," int_or_var(i4) "," int_or_var(i5) "," int_or_var(i6) "as" ident(H) :=
+  specialize oldH as H;
+  especialize H with id1,id2 at i1,i2,i3,i4,i5,i6 .
+Tactic Notation "especialize" constr(H) "with" ident(id1) "," ident(id2) "at" int_or_var(i1) "," int_or_var(i2) "," int_or_var(i3) "," int_or_var(i4) "," int_or_var(i5) "," int_or_var(i6) "as" "?" :=
+  let nme := fresh in
+  especialize H with id1,id2 at i1,i2,i3,i4,i5,i6 as nme.
+
+Tactic Notation "especialize" constr(H) "with" ident(id1) "," ident(id2) "at" int_or_var(i1) "," int_or_var(i2) "," int_or_var(i3) "," int_or_var(i4) "," int_or_var(i5) "," int_or_var(i6) "," int_or_var(i7) :=
+  fail_if_not_hyp H;
+  spec_evar H id1;
+  especialize H with id2 at i1,i2,i3,i4,i5,i6,i7 .
+Tactic Notation "especialize" constr(oldH) "with" ident(id1) "," ident(id2) "at" int_or_var(i1) "," int_or_var(i2) "," int_or_var(i3) "," int_or_var(i4) "," int_or_var(i5) "," int_or_var(i6) "," int_or_var(i7) "as" ident(H) :=
+  specialize oldH as H;
+  especialize H with id1,id2 at i1,i2,i3,i4,i5,i6,i7 .
+Tactic Notation "especialize" constr(H) "with" ident(id1) "," ident(id2) "at" int_or_var(i1) "," int_or_var(i2) "," int_or_var(i3) "," int_or_var(i4) "," int_or_var(i5) "," int_or_var(i6) "," int_or_var(i7) "as" "?" :=
+  let nme := fresh in
+  especialize H with id1,id2 at i1,i2,i3,i4,i5,i6,i7 as nme.
+
+
+Tactic Notation "especialize" constr(H) "with" ident(id1) "," ident(id2) "," ident(id3) "at" "*" :=
+  fail_if_not_hyp H;
+  spec_evar H id1;
+  especialize H with id2,id3 at *.
+Tactic Notation "especialize" constr(oldH) "with" ident(id1) "," ident(id2) "," ident(id3) "at" "*" "as" ident(H) :=
+  specialize oldH as H;
+  especialize H with id1,id2,id3 at *.
+Tactic Notation "especialize" constr(H) "with" ident(id1) "," ident(id2) "," ident(id3) "at" "*" "as" "?" :=
+  let nme := fresh in
+  especialize H with id1,id2,id3 at * as nme.
+
+Tactic Notation "especialize" constr(H) "with" ident(id1) "," ident(id2) "," ident(id3) "until" constr(i) :=
+  fail_if_not_hyp H;
+  spec_evar H id1;
+  especialize H with id2,id3 until i .
+Tactic Notation "especialize" constr(oldH) "with" ident(id1) "," ident(id2) "," ident(id3) "until" constr(i) "as" ident(H) :=
+  specialize oldH as H;
+  especialize H with id1,id2,id3 until i .
+Tactic Notation "especialize" constr(H) "with" ident(id1) "," ident(id2) "," ident(id3) "until" constr(i) "as" "?" :=
+  let nme := fresh in
+  especialize H with id1,id2,id3 until i as nme.
+
+Tactic Notation "especialize" constr(H) "with" ident(id1) "," ident(id2) "," ident(id3) "at" int_or_var(i) :=
+  fail_if_not_hyp H;
+  spec_evar H id1;
+  especialize H with id2,id3 at i .
+Tactic Notation "especialize" constr(oldH) "with" ident(id1) "," ident(id2) "," ident(id3) "at" int_or_var(i) "as" ident(H) :=
+  specialize oldH as H;
+  especialize H with id1,id2,id3 at i .
+Tactic Notation "especialize" constr(H) "with" ident(id1) "," ident(id2) "," ident(id3) "at" int_or_var(i) "as" "?" :=
+  let nme := fresh in
+  especialize H with id1,id2,id3 at i as nme.
+
+Tactic Notation "especialize" constr(H) "with" ident(id1) "," ident(id2) "," ident(id3) "at" int_or_var(i) ":" ident(hprem) :=
+  fail_if_not_hyp H;
+  spec_evar H id1;
+  especialize H with id2,id3 at i : hprem.
+Tactic Notation "especialize" constr(oldH) "with" ident(id1) "," ident(id2) "," ident(id3) "at" int_or_var(i) "as" ident(H) ":" ident(hprem) :=
+  specialize oldH as H;
+  especialize H with id1,id2,id3 at i : hprem.
+Tactic Notation "especialize" constr(H) "with" ident(id1) "," ident(id2) "," ident(id3) "at" int_or_var(i) "as" "?" ":" ident(hprem) :=
+  let nme := fresh in
+  especialize H with id1,id2,id3 at i as nme : hprem.
+
+Tactic Notation "especialize" constr(H) "with" ident(id1) "," ident(id2) "," ident(id3) "at" int_or_var(i1) "," int_or_var(i2) :=
+  fail_if_not_hyp H;
+  spec_evar H id1;
+  especialize H with id2,id3 at i1,i2.
+Tactic Notation "especialize" constr(oldH) "with" ident(id1) "," ident(id2) "," ident(id3) "at" int_or_var(i1) "," int_or_var(i2) "as" ident(H) :=
+  specialize oldH as H;
+  especialize H with id1,id2,id3 at i1,i2 .
+Tactic Notation "especialize" constr(H) "with" ident(id1) "," ident(id2) "," ident(id3) "at" int_or_var(i1) "," int_or_var(i2) "as" "?" :=
+  let nme := fresh in
+  especialize H with id1,id2,id3 at i1,i2 as nme.
+
+Tactic Notation "especialize" constr(H) "with" ident(id1) "," ident(id2) "," ident(id3) "at" int_or_var(i1) "," int_or_var(i2) "," int_or_var(i3) :=
+  fail_if_not_hyp H;
+  spec_evar H id1;
+  especialize H with id2,id3 at i1,i2,i3 .
+Tactic Notation "especialize" constr(oldH) "with" ident(id1) "," ident(id2) "," ident(id3) "at" int_or_var(i1) "," int_or_var(i2) "," int_or_var(i3) "as" ident(H) :=
+  specialize oldH as H;
+  especialize H with id1,id2,id3 at i1,i2,i3 .
+Tactic Notation "especialize" constr(H) "with" ident(id1) "," ident(id2) "," ident(id3) "at" int_or_var(i1) "," int_or_var(i2) "," int_or_var(i3) "as" "?" :=
+  let nme := fresh in
+  especialize H with id1,id2,id3 at i1,i2,i3 as nme.
+
+Tactic Notation "especialize" constr(H) "with" ident(id1) "," ident(id2) "," ident(id3) "at" int_or_var(i1) "," int_or_var(i2)  "," int_or_var(i3) "," int_or_var(i4) :=
+  fail_if_not_hyp H;
+  spec_evar H id1;
+  especialize H with id2,id3 at i1,i2,i3,i4 .
+Tactic Notation "especialize" constr(oldH) "with" ident(id1) "," ident(id2) "," ident(id3) "at" int_or_var(i1) "," int_or_var(i2)  "," int_or_var(i3) "," int_or_var(i4) "as" ident(H) :=
+  specialize oldH as H;
+  especialize H with id1,id2,id3 at i1,i2,i3,i4 .
+Tactic Notation "especialize" constr(H) "with" ident(id1) "," ident(id2) "," ident(id3) "at" int_or_var(i1) "," int_or_var(i2)  "," int_or_var(i3) "," int_or_var(i4) "as" "?" :=
+  let nme := fresh in
+  especialize H with id1,id2,id3 at i1,i2,i3,i4 as nme.
+
+Tactic Notation "especialize" constr(H) "with" ident(id1) "," ident(id2) "," ident(id3) "at" int_or_var(i1) "," int_or_var(i2) "," int_or_var(i3) "," int_or_var(i4) "," int_or_var(i5) :=
+  fail_if_not_hyp H;
+  spec_evar H id1;
+  especialize H with id2,id3 at i1,i2,i3,i4,i5 .
+Tactic Notation "especialize" constr(oldH) "with" ident(id1) "," ident(id2) "," ident(id3) "at" int_or_var(i1) "," int_or_var(i2) "," int_or_var(i3) "," int_or_var(i4) "," int_or_var(i5) "as" ident(H) :=
+  specialize oldH as H;
+  especialize H with id1,id2,id3 at i1,i2,i3,i4,i5 .
+Tactic Notation "especialize" constr(H) "with" ident(id1) "," ident(id2) "," ident(id3) "at" int_or_var(i1) "," int_or_var(i2) "," int_or_var(i3) "," int_or_var(i4) "," int_or_var(i5) "as" "?" :=
+  let nme := fresh in
+  especialize H with id1,id2,id3 at i1,i2,i3,i4,i5 as nme.
+
+Tactic Notation "especialize" constr(H) "with" ident(id1) "," ident(id2) "," ident(id3) "at" int_or_var(i1) "," int_or_var(i2) "," int_or_var(i3) "," int_or_var(i4) "," int_or_var(i5) "," int_or_var(i6) :=
+  fail_if_not_hyp H;
+  spec_evar H id1;
+  especialize H with id2,id3 at i1,i2,i3,i4,i5,i6 .
+Tactic Notation "especialize" constr(oldH) "with" ident(id1) "," ident(id2) "," ident(id3) "at" int_or_var(i1) "," int_or_var(i2) "," int_or_var(i3) "," int_or_var(i4) "," int_or_var(i5) "," int_or_var(i6) "as" ident(H) :=
+  specialize oldH as H;
+  especialize H with id1,id2,id3 at i1,i2,i3,i4,i5,i6 .
+Tactic Notation "especialize" constr(H) "with" ident(id1) "," ident(id2) "," ident(id3) "at" int_or_var(i1) "," int_or_var(i2) "," int_or_var(i3) "," int_or_var(i4) "," int_or_var(i5) "," int_or_var(i6) "as" "?" :=
+  let nme := fresh in
+  especialize H with id1,id2,id3 at i1,i2,i3,i4,i5,i6 as nme.
+
+Tactic Notation "especialize" constr(H) "with" ident(id1) "," ident(id2) "," ident(id3) "at" int_or_var(i1) "," int_or_var(i2) "," int_or_var(i3) "," int_or_var(i4) "," int_or_var(i5) "," int_or_var(i6) "," int_or_var(i7) :=
+  fail_if_not_hyp H;
+  spec_evar H id1;
+  especialize H with id2,id3 at i1,i2,i3,i4,i5,i6,i7 .
+Tactic Notation "especialize" constr(oldH) "with" ident(id1) "," ident(id2) "," ident(id3) "at" int_or_var(i1) "," int_or_var(i2) "," int_or_var(i3) "," int_or_var(i4) "," int_or_var(i5) "," int_or_var(i6) "," int_or_var(i7) "as" ident(H) :=
+  specialize oldH as H;
+  especialize H with id1,id2,id3 at i1,i2,i3,i4,i5,i6,i7 .
+Tactic Notation "especialize" constr(H) "with" ident(id1) "," ident(id2) "," ident(id3) "at" int_or_var(i1) "," int_or_var(i2) "," int_or_var(i3) "," int_or_var(i4) "," int_or_var(i5) "," int_or_var(i6) "," int_or_var(i7) "as" "?" :=
+  let nme := fresh in
+  especialize H with id1,id2,id3 at i1,i2,i3,i4,i5,i6,i7 as nme.
 
 
 
 
-(* TEST *)
+Tactic Notation "especialize" constr(H) "with" ident(id1) "," ident(id2) "," ident(id3) "," ident(id4) "at" "*" :=
+  fail_if_not_hyp H;
+  spec_evar H id1;
+  especialize H with id2,id3,id4 at *.
+Tactic Notation "especialize" constr(oldH) "with" ident(id1) "," ident(id2) "," ident(id3) "," ident(id4) "at" "*" "as" ident(H) :=
+  specialize oldH as H;
+  especialize H with id1,id2,id3,id4 at *.
+Tactic Notation "especialize" constr(H) "with" ident(id1) "," ident(id2) "," ident(id3) "," ident(id4) "at" "*" "as" "?" :=
+  let nme := fresh in
+  especialize H with id1,id2,id3,id4 at * as nme.
 
-Lemma foo: (eq_one 2 -> eq_one 1 -> False) -> False.
-Proof.
-  intros H.
-  especialize (le_sind 0) at 1 as hh : h.
-  { admit. }
-  especialize min_l at 1 as ? : ?.
-  { apply (le_n O). }
-  
-  especialize H at 1 as hh : h.
-  { reflexivity. }
-  match type of h with False => idtac "OK" | _ => fail end.
-  assumption.
-Qed.
-*)
+Tactic Notation "especialize" constr(H) "with" ident(id1) "," ident(id2) "," ident(id3) "," ident(id4) "until" constr(i) :=
+  fail_if_not_hyp H;
+  spec_evar H id1;
+  especialize H with id2,id3,id4 until i .
+Tactic Notation "especialize" constr(oldH) "with" ident(id1) "," ident(id2) "," ident(id3) "," ident(id4) "until" constr(i) "as" ident(H) :=
+  specialize oldH as H;
+  especialize H with id1,id2,id3,id4 until i .
+Tactic Notation "especialize" constr(H) "with" ident(id1) "," ident(id2) "," ident(id3) "," ident(id4) "until" constr(i) "as" "?" :=
+  let nme := fresh in
+  especialize H with id1,id2,id3,id4 until i as nme.
+
+Tactic Notation "especialize" constr(H) "with" ident(id1) "," ident(id2) "," ident(id3) "," ident(id4) "at" int_or_var(i) :=
+  fail_if_not_hyp H;
+  spec_evar H id1;
+  especialize H with id2,id3,id4 at i .
+Tactic Notation "especialize" constr(oldH) "with" ident(id1) "," ident(id2) "," ident(id3) "," ident(id4) "at" int_or_var(i) "as" ident(H) :=
+  specialize oldH as H;
+  especialize H with id1,id2,id3,id4 at i .
+Tactic Notation "especialize" constr(H) "with" ident(id1) "," ident(id2) "," ident(id3) "," ident(id4) "at" int_or_var(i) "as" "?" :=
+  let nme := fresh in
+  especialize H with id1,id2,id3,id4 at i as nme.
+
+Tactic Notation "especialize" constr(H) "with" ident(id1) "," ident(id2) "," ident(id3) "," ident(id4) "at" int_or_var(i) ":" ident(hprem) :=
+  fail_if_not_hyp H;
+  spec_evar H id1;
+  especialize H with id2,id3,id4 at i : hprem.
+Tactic Notation "especialize" constr(oldH) "with" ident(id1) "," ident(id2) "," ident(id3) "," ident(id4) "at" int_or_var(i) "as" ident(H) ":" ident(hprem) :=
+  specialize oldH as H;
+  especialize H with id1,id2,id3,id4 at i : hprem.
+Tactic Notation "especialize" constr(H) "with" ident(id1) "," ident(id2) "," ident(id3) "," ident(id4) "at" int_or_var(i) "as" "?" ":" ident(hprem) :=
+  let nme := fresh in
+  especialize H with id1,id2,id3,id4 at i as nme : hprem.
+
+Tactic Notation "especialize" constr(H) "with" ident(id1) "," ident(id2) "," ident(id3) "," ident(id4) "at" int_or_var(i1) "," int_or_var(i2) :=
+  fail_if_not_hyp H;
+  spec_evar H id1;
+  especialize H with id2,id3,id4 at i1,i2 .
+Tactic Notation "especialize" constr(oldH) "with" ident(id1) "," ident(id2) "," ident(id3) "," ident(id4) "at" int_or_var(i1) "," int_or_var(i2) "as" ident(H) :=
+  specialize oldH as H;
+  especialize H with id1,id2,id3,id4 at i1,i2 .
+Tactic Notation "especialize" constr(H) "with" ident(id1) "," ident(id2) "," ident(id3) "," ident(id4) "at" int_or_var(i1) "," int_or_var(i2) "as" "?" :=
+  let nme := fresh in
+  especialize H with id1,id2,id3,id4 at i1,i2 as nme.
+
+Tactic Notation "especialize" constr(H) "with" ident(id1) "," ident(id2) "," ident(id3) "," ident(id4) "at" int_or_var(i1) "," int_or_var(i2) "," int_or_var(i3) :=
+  fail_if_not_hyp H;
+  spec_evar H id1;
+  especialize H with id2,id3,id4 at i1,i2,i3 .
+Tactic Notation "especialize" constr(oldH) "with" ident(id1) "," ident(id2) "," ident(id3) "," ident(id4) "at" int_or_var(i1) "," int_or_var(i2) "," int_or_var(i3) "as" ident(H) :=
+  specialize oldH as H;
+  especialize H with id1,id2,id3,id4 at i1,i2,i3 .
+Tactic Notation "especialize" constr(H) "with" ident(id1) "," ident(id2) "," ident(id3) "," ident(id4) "at" int_or_var(i1) "," int_or_var(i2) "," int_or_var(i3) "as" "?" :=
+  let nme := fresh in
+  especialize H with id1,id2,id3,id4 at i1,i2,i3 as nme.
+
+Tactic Notation "especialize" constr(H) "with" ident(id1) "," ident(id2) "," ident(id3) "," ident(id4) "at" int_or_var(i1) "," int_or_var(i2)  "," int_or_var(i3) "," int_or_var(i4) :=
+  fail_if_not_hyp H;
+  spec_evar H id1;
+  especialize H with id2,id3,id4 at i1,i2,i3,i4 .
+Tactic Notation "especialize" constr(oldH) "with" ident(id1) "," ident(id2) "," ident(id3) "," ident(id4) "at" int_or_var(i1) "," int_or_var(i2)  "," int_or_var(i3) "," int_or_var(i4) "as" ident(H) :=
+  specialize oldH as H;
+  especialize H with id1,id2,id3,id4 at i1,i2,i3,i4 .
+Tactic Notation "especialize" constr(H) "with" ident(id1) "," ident(id2) "," ident(id3) "," ident(id4) "at" int_or_var(i1) "," int_or_var(i2)  "," int_or_var(i3) "," int_or_var(i4) "as" "?" :=
+  let nme := fresh in
+  especialize H with id1,id2,id3,id4 at i1,i2,i3,i4 as nme.
+
+Tactic Notation "especialize" constr(H) "with" ident(id1) "," ident(id2) "," ident(id3) "," ident(id4) "at" int_or_var(i1) "," int_or_var(i2) "," int_or_var(i3) "," int_or_var(i4) "," int_or_var(i5) :=
+  fail_if_not_hyp H;
+  spec_evar H id1;
+  especialize H with id2,id3,id4 at i1,i2,i3,i4,i5 .
+Tactic Notation "especialize" constr(oldH) "with" ident(id1) "," ident(id2) "," ident(id3) "," ident(id4) "at" int_or_var(i1) "," int_or_var(i2) "," int_or_var(i3) "," int_or_var(i4) "," int_or_var(i5) "as" ident(H) :=
+  specialize oldH as H;
+  especialize H with id1,id2,id3,id4 at i1,i2,i3,i4,i5 .
+Tactic Notation "especialize" constr(H) "with" ident(id1) "," ident(id2) "," ident(id3) "," ident(id4) "at" int_or_var(i1) "," int_or_var(i2) "," int_or_var(i3) "," int_or_var(i4) "," int_or_var(i5) "as" "?" :=
+  let nme := fresh in
+  especialize H with id1,id2,id3,id4 at i1,i2,i3,i4,i5 as nme.
+
+Tactic Notation "especialize" constr(H) "with" ident(id1) "," ident(id2) "," ident(id3) "," ident(id4) "at" int_or_var(i1) "," int_or_var(i2) "," int_or_var(i3) "," int_or_var(i4) "," int_or_var(i5) "," int_or_var(i6) :=
+  fail_if_not_hyp H;
+  spec_evar H id1;
+  especialize H with id2,id3,id4 at i1,i2,i3,i4,i5,i6 .
+Tactic Notation "especialize" constr(oldH) "with" ident(id1) "," ident(id2) "," ident(id3) "," ident(id4) "at" int_or_var(i1) "," int_or_var(i2) "," int_or_var(i3) "," int_or_var(i4) "," int_or_var(i5) "," int_or_var(i6) "as" ident(H) :=
+  specialize oldH as H;
+  especialize H with id1,id2,id3,id4 at i1,i2,i3,i4,i5,i6 .
+Tactic Notation "especialize" constr(H) "with" ident(id1) "," ident(id2) "," ident(id3) "," ident(id4) "at" int_or_var(i1) "," int_or_var(i2) "," int_or_var(i3) "," int_or_var(i4) "," int_or_var(i5) "," int_or_var(i6) "as" "?" :=
+  let nme := fresh in
+  especialize H with id1,id2,id3,id4 at i1,i2,i3,i4,i5,i6 as nme.
+
+Tactic Notation "especialize" constr(H) "with" ident(id1) "," ident(id2) "," ident(id3) "," ident(id4) "at" int_or_var(i1) "," int_or_var(i2) "," int_or_var(i3) "," int_or_var(i4) "," int_or_var(i5) "," int_or_var(i6) "," int_or_var(i7) :=
+  fail_if_not_hyp H;
+  spec_evar H id1;
+  especialize H with id2,id3,id4 at i1,i2,i3,i4,i5,i6,i7 .
+Tactic Notation "especialize" constr(oldH) "with" ident(id1) "," ident(id2) "," ident(id3) "," ident(id4) "at" int_or_var(i1) "," int_or_var(i2) "," int_or_var(i3) "," int_or_var(i4) "," int_or_var(i5) "," int_or_var(i6) "," int_or_var(i7) "as" ident(H) :=
+  specialize oldH as H;
+  especialize H with id1,id2,id3,id4 at i1,i2,i3,i4,i5,i6,i7 .
+Tactic Notation "especialize" constr(H) "with" ident(id1) "," ident(id2) "," ident(id3) "," ident(id4) "at" int_or_var(i1) "," int_or_var(i2) "," int_or_var(i3) "," int_or_var(i4) "," int_or_var(i5) "," int_or_var(i6) "," int_or_var(i7) "as" "?" :=
+  let nme := fresh in
+  especialize H with id1,id2,id3,id4 at i1,i2,i3,i4,i5,i6,i7 as nme.
 
 
+
+
+Tactic Notation "especialize" constr(H) "with" ident(id1) "," ident(id2) "," ident(id3) "," ident(id4) "," ident(id5) "at" "*" :=
+  fail_if_not_hyp H;
+  spec_evar H id1;
+  especialize H with id2,id3,id4,id5 at *.
+Tactic Notation "especialize" constr(oldH) "with" ident(id1) "," ident(id2) "," ident(id3) "," ident(id4) "," ident(id5) "at" "*" "as" ident(H) :=
+  specialize oldH as H;
+  especialize H with id1,id2,id3,id4,id5 at *.
+Tactic Notation "especialize" constr(H) "with" ident(id1) "," ident(id2) "," ident(id3) "," ident(id4) "," ident(id5) "at" "*" "as" "?" :=
+  let nme := fresh in
+  especialize H with id1,id2,id3,id4,id5 at * as nme.
+
+Tactic Notation "especialize" constr(H) "with" ident(id1) "," ident(id2) "," ident(id3) "," ident(id4) "," ident(id5) "until" constr(i) :=
+  fail_if_not_hyp H;
+  spec_evar H id1;
+  especialize H with id2,id3,id4,id5 until i.
+Tactic Notation "especialize" constr(oldH) "with" ident(id1) "," ident(id2) "," ident(id3) "," ident(id4) "," ident(id5) "until" constr(i) "as" ident(H) :=
+  specialize oldH as H;
+  especialize H with id1,id2,id3,id4,id5 until i .
+Tactic Notation "especialize" constr(H) "with" ident(id1) "," ident(id2) "," ident(id3) "," ident(id4) "," ident(id5) "until" constr(i) "as" "?" :=
+  let nme := fresh in
+  especialize H with id1,id2,id3,id4,id5 until i as nme.
+
+Tactic Notation "especialize" constr(H) "with" ident(id1) "," ident(id2) "," ident(id3) "," ident(id4) "," ident(id5) "at" int_or_var(i) :=
+  fail_if_not_hyp H;
+  spec_evar H id1;
+  especialize H with id2,id3,id4,id5 at i .
+Tactic Notation "especialize" constr(oldH) "with" ident(id1) "," ident(id2) "," ident(id3) "," ident(id4) "," ident(id5) "at" int_or_var(i) "as" ident(H) :=
+  specialize oldH as H;
+  especialize H with id1,id2,id3,id4,id5 at i .
+Tactic Notation "especialize" constr(H) "with" ident(id1) "," ident(id2) "," ident(id3) "," ident(id4) "," ident(id5) "at" int_or_var(i) "as" "?" :=
+  let nme := fresh in
+  especialize H with id1,id2,id3,id4,id5 at i as nme.
+
+Tactic Notation "especialize" constr(H) "with" ident(id1) "," ident(id2) "," ident(id3) "," ident(id4) "," ident(id5) "at" int_or_var(i) ":" ident(hprem) :=
+  fail_if_not_hyp H;
+  spec_evar H id1;
+  especialize H with id2,id3,id4,id5 at i : hprem.
+Tactic Notation "especialize" constr(oldH) "with" ident(id1) "," ident(id2) "," ident(id3) "," ident(id4) "," ident(id5) "at" int_or_var(i) "as" ident(H) ":" ident(hprem) :=
+  specialize oldH as H;
+  especialize H with id1,id2,id3,id4,id5 at i : hprem.
+Tactic Notation "especialize" constr(H) "with" ident(id1) "," ident(id2) "," ident(id3) "," ident(id4) "," ident(id5) "at" int_or_var(i) "as" "?" ":" ident(hprem) :=
+  let nme := fresh in
+  especialize H with id1,id2,id3,id4,id5 at i as nme : hprem.
+
+Tactic Notation "especialize" constr(H) "with" ident(id1) "," ident(id2) "," ident(id3) "," ident(id4) "," ident(id5) "at" int_or_var(i1) "," int_or_var(i2) :=
+  fail_if_not_hyp H;
+  spec_evar H id1;
+  especialize H with id2,id3,id4,id5 at i1,i2 .
+Tactic Notation "especialize" constr(oldH) "with" ident(id1) "," ident(id2) "," ident(id3) "," ident(id4) "," ident(id5) "at" int_or_var(i1) "," int_or_var(i2) "as" ident(H) :=
+  specialize oldH as H;
+  especialize H with id1,id2,id3,id4,id5 at i1,i2 .
+Tactic Notation "especialize" constr(H) "with" ident(id1) "," ident(id2) "," ident(id3) "," ident(id4) "," ident(id5) "at" int_or_var(i1) "," int_or_var(i2) "as" "?" :=
+  let nme := fresh in
+  especialize H with id1,id2,id3,id4,id5 at i1,i2 as nme.
+
+Tactic Notation "especialize" constr(H) "with" ident(id1) "," ident(id2) "," ident(id3) "," ident(id4) "," ident(id5) "at" int_or_var(i1) "," int_or_var(i2) :=
+  fail_if_not_hyp H;
+  spec_evar H id1;
+  especialize H with id2,id3,id4,id5 at i1,i2 .
+Tactic Notation "especialize" constr(oldH) "with" ident(id1) "," ident(id2) "," ident(id3) "," ident(id4) "," ident(id5) "at" int_or_var(i1) "," int_or_var(i2) "as" ident(H) :=
+  specialize oldH as H;
+  especialize H with id1,id2,id3,id4,id5 at i1,i2 .
+Tactic Notation "especialize" constr(H) "with" ident(id1) "," ident(id2) "," ident(id3) "," ident(id4) "," ident(id5) "at" int_or_var(i1) "," int_or_var(i2) "as" "?" :=
+  let nme := fresh in
+  especialize H with id1,id2,id3,id4,id5 at i1,i2 as nme.
+
+Tactic Notation "especialize" constr(H) "with" ident(id1) "," ident(id2) "," ident(id3) "," ident(id4) "," ident(id5) "at" int_or_var(i1) "," int_or_var(i2) "," int_or_var(i3) :=
+  fail_if_not_hyp H;
+  spec_evar H id1;
+  especialize H with id2,id3,id4,id5 at i1,i2,i3 .
+Tactic Notation "especialize" constr(oldH) "with" ident(id1) "," ident(id2) "," ident(id3) "," ident(id4) "," ident(id5) "at" int_or_var(i1) "," int_or_var(i2) "," int_or_var(i3) "as" ident(H) :=
+  specialize oldH as H;
+  especialize H with id1,id2,id3,id4,id5 at i1,i2,i3 .
+Tactic Notation "especialize" constr(H) "with" ident(id1) "," ident(id2) "," ident(id3) "," ident(id4) "," ident(id5) "at" int_or_var(i1) "," int_or_var(i2) "," int_or_var(i3) "as" "?" :=
+  let nme := fresh in
+  especialize H with id1,id2,id3,id4,id5 at i1,i2,i3 as nme.
+
+Tactic Notation "especialize" constr(H) "with" ident(id1) "," ident(id2) "," ident(id3) "," ident(id4) "," ident(id5) "at" int_or_var(i1) "," int_or_var(i2)  "," int_or_var(i3) "," int_or_var(i4) :=
+  fail_if_not_hyp H;
+  spec_evar H id1;
+  especialize H with id2,id3,id4,id5 at i1,i2,i3,i4 .
+Tactic Notation "especialize" constr(oldH) "with" ident(id1) "," ident(id2) "," ident(id3) "," ident(id4) "," ident(id5) "at" int_or_var(i1) "," int_or_var(i2)  "," int_or_var(i3) "," int_or_var(i4) "as" ident(H) :=
+  specialize oldH as H;
+  especialize H with id1,id2,id3,id4,id5 at i1,i2,i3,i4 .
+Tactic Notation "especialize" constr(H) "with" ident(id1) "," ident(id2) "," ident(id3) "," ident(id4) "," ident(id5) "at" int_or_var(i1) "," int_or_var(i2)  "," int_or_var(i3) "," int_or_var(i4) "as" "?" :=
+  let nme := fresh in
+  especialize H with id1,id2,id3,id4,id5 at i1,i2,i3,i4 as nme.
+
+Tactic Notation "especialize" constr(H) "with" ident(id1) "," ident(id2) "," ident(id3) "," ident(id4) "," ident(id5) "at" int_or_var(i1) "," int_or_var(i2) "," int_or_var(i3) "," int_or_var(i4) "," int_or_var(i5) :=
+  fail_if_not_hyp H;
+  spec_evar H id1;
+  especialize H with id2,id3,id4,id5 at i1,i2,i3,i4,i5 .
+Tactic Notation "especialize" constr(oldH) "with" ident(id1) "," ident(id2) "," ident(id3) "," ident(id4) "," ident(id5) "at" int_or_var(i1) "," int_or_var(i2) "," int_or_var(i3) "," int_or_var(i4) "," int_or_var(i5) "as" ident(H) :=
+  specialize oldH as H;
+  especialize H with id1,id2,id3,id4,id5 at i1,i2,i3,i4,i5 .
+Tactic Notation "especialize" constr(H) "with" ident(id1) "," ident(id2) "," ident(id3) "," ident(id4) "," ident(id5) "at" int_or_var(i1) "," int_or_var(i2) "," int_or_var(i3) "," int_or_var(i4) "," int_or_var(i5) "as" "?" :=
+  let nme := fresh in
+  especialize H with id1,id2,id3,id4,id5 at i1,i2,i3,i4,i5 as nme.
+
+Tactic Notation "especialize" constr(H) "with" ident(id1) "," ident(id2) "," ident(id3) "," ident(id4) "," ident(id5) "at" int_or_var(i1) "," int_or_var(i2) "," int_or_var(i3) "," int_or_var(i4) "," int_or_var(i5) "," int_or_var(i6) :=
+  fail_if_not_hyp H;
+  spec_evar H id1;
+  especialize H with id2,id3,id4,id5 at i1,i2,i3,i4,i5,i6 .
+Tactic Notation "especialize" constr(oldH) "with" ident(id1) "," ident(id2) "," ident(id3) "," ident(id4) "," ident(id5) "at" int_or_var(i1) "," int_or_var(i2) "," int_or_var(i3) "," int_or_var(i4) "," int_or_var(i5) "," int_or_var(i6) "as" ident(H) :=
+  specialize oldH as H;
+  especialize H with id1,id2,id3,id4,id5 at i1,i2,i3,i4,i5,i6 .
+Tactic Notation "especialize" constr(H) "with" ident(id1) "," ident(id2) "," ident(id3) "," ident(id4) "," ident(id5) "at" int_or_var(i1) "," int_or_var(i2) "," int_or_var(i3) "," int_or_var(i4) "," int_or_var(i5) "," int_or_var(i6) "as" "?" :=
+  let nme := fresh in
+  especialize H with id1,id2,id3,id4,id5 at i1,i2,i3,i4,i5,i6 as nme.
+
+Tactic Notation "especialize" constr(H) "with" ident(id1) "," ident(id2) "," ident(id3) "," ident(id4) "," ident(id5) "at" int_or_var(i1) "," int_or_var(i2) "," int_or_var(i3) "," int_or_var(i4) "," int_or_var(i5) "," int_or_var(i6) "," int_or_var(i7) :=
+  fail_if_not_hyp H;
+  spec_evar H id1;
+  especialize H with id2,id3,id4,id5 at i1,i2,i3,i4,i5,i6,i7 .
+Tactic Notation "especialize" constr(oldH) "with" ident(id1) "," ident(id2) "," ident(id3) "," ident(id4) "," ident(id5) "at" int_or_var(i1) "," int_or_var(i2) "," int_or_var(i3) "," int_or_var(i4) "," int_or_var(i5) "," int_or_var(i6) "," int_or_var(i7) "as" ident(H) :=
+  specialize oldH as H;
+  especialize H with id1,id2,id3,id4,id5 at i1,i2,i3,i4,i5,i6,i7 .
+Tactic Notation "especialize" constr(H) "with" ident(id1) "," ident(id2) "," ident(id3) "," ident(id4) "," ident(id5) "at" int_or_var(i1) "," int_or_var(i2) "," int_or_var(i3) "," int_or_var(i4) "," int_or_var(i5) "," int_or_var(i6) "," int_or_var(i7) "as" "?" :=
+  let nme := fresh in
+  especialize H with id1,id2,id3,id4,id5 at i1,i2,i3,i4,i5,i6,i7 as nme.
 
