LibHyps/LibHypsRegression.v
@@ -118,255 +118,559 @@ Lemma dummy: forall x y,
 Qed. 
 
 
-(* BROKEN IN 8.18 *)
-(*
 Definition eq_one (i:nat) := i = 1.
-(* eq_one is delta_reducible but I don't want it to be reduced. *)
-Lemma test_espec: (eq_one 2 -> eq_one 3 -> eq_one 1 -> False) -> True.
-Proof.
-  intros h_eqone.
-  (* let nme := fresh_robust H "hh" "def" in idtac nme.Definition *)
+Module AS.
 
-  especialize h_eqone as newH at 2;
-    [ admit | match type of newH with eq_one 2 -> eq_one 1 -> False => idtac end;
-              match type of h_eqone with  eq_one 2 -> eq_one 3 -> eq_one 1 -> False => idtac end].
-  Undo.
-  especialize h_eqone at 2 as newH;
-    [ admit | match type of newH with eq_one 2 -> eq_one 1 -> False => idtac end;
-              match type of h_eqone with  eq_one 2 -> eq_one 3 -> eq_one 1 -> False => idtac end].
-  Undo.
 
-  especialize (let x:=Nat.le_antisymm in x) at 2 as hhh;
-    [ admit | match type of hhh with _ <= _ -> _ = _ => idtac | _ => fail "Test failed!" end ].
-  Undo.
+  Lemma test_espec: forall x:nat, x = 1 -> (x = 1 -> False) -> x > 1.
+  Proof.
+    intros x hx h_eqone.
+    especialize h_eqone at 1 .
+    + assumption.
+    + match type of h_eqone with
+        False => idtac
+      | _ => fail "test failed!"
+      end.
+      contradiction.
+  Qed.
 
-  especialize (let x:=Nat.le_antisymm in x)as hhh at 2;
-    [ admit | match type of hhh with _ <= _ -> _ = _ => idtac | _ => fail "Test failed!" end ].
-  Undo.
+  Lemma test_espec2: forall x:nat, x = 1 -> (x = 1 -> False) -> x > 1.
+  Proof.
+    intros x hx h_eqone.
+    especialize h_eqone at 1 as h.
+    + assumption.
+    + match type of h with
+        False => idtac
+      | _ => fail "test failed!"
+      end.
+      contradiction.
+  Qed.
 
-  especialize h_eqone at 2;
-    [ admit | match type of h_eqone with eq_one 2 -> eq_one 1 -> False => idtac end].
-  Undo.
+  Lemma test_espec3: forall x:nat, x = 1 -> (x = 1 -> False) -> x > 1.
+  Proof.
+    intros x hx h_eqone.
+    especialize h_eqone at 1 as ?.
+    + assumption.
+    + match type of H with
+        False => idtac
+      | _ => fail "test failed!"
+      end.
+      contradiction.
+  Qed.
 
-  especialize (let x:=Nat.le_antisymm in x) at 2;
-    [ admit | match goal with |- (_ <= _ -> _ = _) -> True => idtac | _ => fail "Test failed!" end ].
-  Undo.
+  Lemma test_espec4: forall x:nat, x = 1 -> (x = 1 -> x = x -> False) -> x > 1.
+  Proof.
+    intros x hx h_eqone.
+    especialize h_eqone at 1,2 as ?.
+    + assumption.
+    + reflexivity.
+    + match type of H with
+        False => idtac
+      | _ => fail "test failed!"
+      end.
+      contradiction.
+  Qed.
 
-  especialize h_eqone as ? at 2;
-    [ admit | match type of h_eqone_spec with eq_one 2 -> eq_one 1 -> False => idtac | _ => fail "Test failed!" end;
-              match type of h_eqone with eq_one 2 -> eq_one 3 -> eq_one 1 -> False => idtac | _ => fail "Test failed!" end].
-  Undo.
-  especialize h_eqone at 2 as ? ;
-    [ admit | match type of h_eqone_spec with eq_one 2 -> eq_one 1 -> False => idtac | _ => fail "Test failed!" end;
-              match type of h_eqone with eq_one 2 -> eq_one 3 -> eq_one 1 -> False => idtac | _ => fail "Test failed!" end].
-  Undo.
+  Lemma test_espec5: forall x:nat, x = 1 -> (x = 1 -> x = x -> x = x -> False) -> x > 1.
+  Proof.
+    intros x hx h_eqone.
+    especialize h_eqone at 1,2,3 as ?.
+    + assumption.
+    + reflexivity.
+    + reflexivity.
+    + match type of H with
+        False => idtac
+      | _ => fail "test failed!"
+      end.
+      contradiction.
+  Qed.
+
   
-  especialize (let x:=Nat.le_antisymm in x) as ? at 2;
-    [ admit | match type of H_spec with _ <= _ -> _ = _ => idtac | _ => fail "Test failed!" end;
-              match type of h_eqone with eq_one 2 -> eq_one 3 -> eq_one 1 -> False => idtac | _ => fail "Test failed!" end].
-  Undo.
-
-  especialize (let x:=Nat.le_antisymm in x) at 2 as ? ;
-    [ admit | match type of H_spec with _ <= _ -> _ = _ => idtac | _ => fail "Test failed!" end;
-              match type of h_eqone with eq_one 2 -> eq_one 3 -> eq_one 1 -> False => idtac | _ => fail "Test failed!" end].
-  Undo.
-
-  especialize h_eqone at 2 : h;
-    [ admit | match type of h_eqone with eq_one 2 -> eq_one 1 -> False => idtac | _ => fail "Test failed!" end;
-              match type of h with 3=1 => idtac | _ => fail "Test failed!" end].
-  Undo.
-
-  especialize (let x:=Nat.le_antisymm in x) at 2 : h;
-    [ admit | match goal with |- (_ <= _ -> _ = _) -> True => idtac | _ => fail "Test failed!" end;
-              match type of h with _ <= _ => idtac | _ => fail "Test failed!" end].
-  Undo.
-
-  especialize h_eqone at 2 : ? ;
-    [ admit | match type of h_eqone with eq_one 2 -> eq_one 1 -> False => idtac | _ => fail "Test failed!" end;
-              match type of h_eqone_prem with 3=1 => idtac | _ => fail "Test failed!" end].
-  Undo. 
-
-  especialize (let x:=Nat.le_antisymm in x) at 2 : ? ;
-    [ admit | match goal with |- (_ <= _ -> _ = _) -> True => idtac | _ => fail "Test failed!" end;
-              match type of H_prem with _ <= _ => idtac | _ => fail "Test failed!" end].
-  Undo.
+  Lemma test_espec_h: forall x:nat, x = 1 -> (forall a y z:nat, x = 1 -> y = 1 -> z+y+a = 2 -> z+1 = x -> False) -> x > 1.
+  Proof.
+    intros x hx h_eqone.
+    especialize h_eqone with a,y at 2,1 as h.
+    + reflexivity.
+    + assumption.
+    + exfalso.
+      apply h with 0.
+      * reflexivity.
+      * symmetry.
+        assumption.
+  Qed.
 
 
-  especialize h_eqone at 2 as newH : h;
-    [ admit | match type of newH with eq_one 2 -> eq_one 1 -> False => idtac | _ => fail "Test failed!" end;
-              match type of h with 3=1 => idtac | _ => fail "Test failed!" end].
-  Undo.
+  
+  Lemma test_espec_h2: forall x:nat, x = 1 -> (forall a y z:nat, a = 1 -> y = 1 -> z+y+a = 2 -> z+1 = x -> False) -> x > 1.
+  Proof.
+    intros x hx h_eqone.
+    especialize h_eqone with a,y at 2,1 as ?.
+    + reflexivity.
+    + reflexivity.
+    + exfalso.
+      apply H with 0.
+      * reflexivity.
+      * symmetry.
+        assumption.
+  Qed.
+  
+End AS.
 
-  especialize (let x:=Nat.le_antisymm in x) at 2 as newH : h;
-    [ admit | match type of newH with (_ <= _ -> _ = _) => idtac | _ => fail "Test failed!" end;
-              match type of h with _ <= _ => idtac | _ => fail "Test failed!" end].
-  Undo.
 
-  especialize h_eqone as newH at 2 : h;
-    [ admit | match type of newH with eq_one 2 -> eq_one 1 -> False => idtac | _ => fail "Test failed!" end;
-              match type of h with 3=1 => idtac | _ => fail "Test failed!" end].
-  Undo.
+Module Using.
 
-  especialize (let x:=Nat.le_antisymm in x) as newH at 2 : h;
-    [ admit |
-      match type of newH with (_ <= _ -> _ = _) => idtac | _ => fail "Test failed!" end;
-      match type of h with _ <= _ => idtac | _ => fail "Test failed!" end].
-  Undo.
+  Lemma test_espec: forall x:nat, x = 1 -> (forall a y z:nat, a = 1 -> y = 1 -> z+y+a = 2 -> z+1 = x -> False) -> x > 1.
+  Proof.
+    intros x hx h_eqone.
+    especialize h_eqone with a,y at 2,1 .
+    + reflexivity.
+    + reflexivity.
+    + exfalso.
+      apply h_eqone with 0.
+      * reflexivity.
+      * symmetry.
+        assumption.
+  Qed.
+  
+  Lemma test_espec_h: forall x:nat, x = 1 -> (forall a y z:nat, a = 1 -> y = 1 -> z+y+a = 2 -> z+1 = x -> False) -> x > 1.
+  Proof.
+    intros x hx h_eqone.
+    especialize h_eqone with a,y at 2,1 as h.
+    + reflexivity.
+    + reflexivity.
+    + exfalso.
+      apply h with 0.
+      * reflexivity.
+      * symmetry.
+        assumption.
+  Qed.
+  
+  Lemma test_espec_h2: forall x:nat, x = 1 -> (forall a y z:nat, a = 1 -> y = 1 -> z+y+a = 2 -> z+1 = x -> False) -> x > 1.
+  Proof.
+    intros x hx h_eqone.
+    especialize h_eqone with a,y at 2,1 as ?.
+    + reflexivity.
+    + reflexivity.
+    + exfalso.
+      apply H with 0.
+      * reflexivity.
+      * symmetry.
+        assumption.
+  Qed.
+  
 
-  especialize h_eqone at 2 as ? : h;
-    [ admit | match type of h_eqone_spec with eq_one 2 -> eq_one 1 -> False => idtac | _ => fail "Test failed!" end;
-              match type of h with 3=1 => idtac | _ => fail "Test failed!" end].
-  Undo.
+  Lemma test_espec2: forall x:nat, x = 1 -> (forall a y z:nat, a = 1 -> y = 1 -> z+y+a = 2 -> z+1 = x -> False) -> x > 1.
+  Proof.
+    intros x hx h_eqone.
+    especialize h_eqone with y at 2 .
+    + reflexivity.
+    + exfalso.
+      apply h_eqone with 1 0.
+      * reflexivity.
+      * reflexivity.
+      * symmetry.
+        assumption.
+  Qed.
+  Lemma test_espec2_h: forall x:nat, x = 1 -> (forall a y z:nat, a = 1 -> y = 1 -> z+y+a = 2 -> z+1 = x -> False) -> x > 1.
+  Proof.
+    intros x hx h_eqone.
+    especialize h_eqone with y at 2 as h.
+    + reflexivity.
+    + exfalso.
+      apply h with 1 0.
+      * reflexivity.
+      * reflexivity.
+      * symmetry.
+        assumption.
+  Qed.
+  Lemma test_espec2_h2: forall x:nat, x = 1 -> (forall a y z:nat, a = 1 -> y = 1 -> z+y+a = 2 -> z+1 = x -> False) -> x > 1.
+  Proof.
+    intros x hx h_eqone.
+    especialize h_eqone with y at 2 as ?.
+    + reflexivity.
+    + exfalso.
+      apply H with 1 0.
+      * reflexivity.
+      * reflexivity.
+      * symmetry.
+        assumption.
+  Qed.
+  
 
-  especialize (let x:=Nat.le_antisymm in x) at 2 as ? : h;
-    [ admit |
-      match type of H_spec with (_ <= _ -> _ = _) => idtac | _ => fail "Test failed!" end;
-      match type of h with _ <= _ => idtac | _ => fail "Test failed!" end].
-  Undo.
+  Lemma test_espec3: forall x:nat, x = 1 -> (forall a y z:nat, a = 1 -> y = 1 -> z+y+a = 2 -> z+1 = x -> False) -> x > 1.
+  Proof.
+    intros x hx h_eqone.
+    especialize h_eqone with y , z at 2 .
+    + reflexivity.
+    + exfalso.
+      apply h_eqone with 1.
+      * reflexivity.
+      * instantiate (z:=0). reflexivity.
+      * symmetry.
+        assumption.
+  Qed.
+  Lemma test_espec3_h: forall x:nat, x = 1 -> (forall a y z:nat, a = 1 -> y = 1 -> z+y+a = 2 -> z+1 = x -> False) -> x > 1.
+  Proof.
+    intros x hx h_eqone.
+    especialize h_eqone with y , z at 2 as h.
+    + reflexivity.
+    + exfalso.
+      apply h with 1.
+      * reflexivity.
+      * instantiate (z:=0). reflexivity.
+      * symmetry.
+        assumption.
+  Qed.
+  Lemma test_espec3_h2: forall x:nat, x = 1 -> (forall a y z:nat, a = 1 -> y = 1 -> z+y+a = 2 -> z+1 = x -> False) -> x > 1.
+  Proof.
+    intros x hx h_eqone.
+    especialize h_eqone with y , z at 2 as ?.
+    + reflexivity.
+    + exfalso.
+      apply H with 1.
+      * reflexivity.
+      * instantiate (z:=0). reflexivity.
+      * symmetry.
+        assumption.
+  Qed.
+  
 
-  especialize h_eqone as ? at 2 : h;
-    [ admit | match type of h_eqone_spec with eq_one 2 -> eq_one 1 -> False => idtac | _ => fail "Test failed!" end;
-              match type of h with 3=1 => idtac | _ => fail "Test failed!" end].
-  Undo.
+  Lemma test_espec4: forall x:nat, x = 1 -> (forall a y z:nat, a = 1 -> y = 1 -> z+y+a = 2 -> z+1 = x -> False) -> x > 1.
+  Proof.
+    intros x hx h_eqone.
+    especialize h_eqone with a, y, z at 1 .
+    + reflexivity.
+    + exfalso.
+      apply h_eqone.
+      * reflexivity.
+      * instantiate (z:=0). reflexivity.
+      * symmetry.
+        assumption.
+  Qed.
+  Lemma test_espec4_h: forall x:nat, x = 1 -> (forall a y z:nat, a = 1 -> y = 1 -> z+y+a = 2 -> z+1 = x -> False) -> x > 1.
+  Proof.
+    intros x hx h_eqone.
+    especialize h_eqone with a, y, z at 1 as h.
+    + reflexivity.
+    + exfalso.
+      apply h.
+      * reflexivity.
+      * instantiate (z:=0). reflexivity.
+      * symmetry.
+        assumption.
+  Qed.
+  Lemma test_espec4_h2: forall x:nat, x = 1 -> (forall a y z:nat, a = 1 -> y = 1 -> z+y+a = 2 -> z+1 = x -> False) -> x > 1.
+  Proof.
+    intros x hx h_eqone.
+    especialize h_eqone with a, y, z at 1 as ?.
+    + reflexivity.
+    + exfalso.
+      apply H.
+      * reflexivity.
+      * instantiate (z:=0). reflexivity.
+      * symmetry.
+        assumption.
+  Qed.
+  
+  Lemma test_espec5: forall x:nat, x = 1 -> (forall a y z:nat, a = 1 -> y = 1 -> z+y+a = 2 -> z+1 = x -> False) -> x > 1.
+  Proof.
+    intros x hx h_eqone.
+    especialize h_eqone with a,y,z at 1 .
+    + reflexivity.
+    + exfalso.
+      apply h_eqone.
+      * reflexivity.
+      * instantiate (z:=0). reflexivity.
+      * symmetry.
+        assumption.
+  Qed.
+  Lemma test_espec5_h: forall x:nat, x = 1 -> (forall a y z:nat, a = 1 -> y = 1 -> z+y+a = 2 -> z+1 = x -> False) -> x > 1.
+  Proof.
+    intros x hx h_eqone.
+    especialize h_eqone with a,y,z at 1 as h.
+    + reflexivity.
+    + exfalso.
+      apply h.
+      * reflexivity.
+      * instantiate (z:=0). reflexivity.
+      * symmetry.
+        assumption.
+  Qed.
+  Lemma test_espec5_h2: forall x:nat, x = 1 -> (forall a y z:nat, a = 1 -> y = 1 -> z+y+a = 2 -> z+1 = x -> False) -> x > 1.
+  Proof.
+    intros x hx h_eqone.
+    especialize h_eqone with a,y,z at 1 as ?.
+    + reflexivity.
+    + exfalso.
+      apply H.
+      * reflexivity.
+      * instantiate (z:=0). reflexivity.
+      * symmetry.
+        assumption.
+  Qed.
+  
+  Lemma test_espec6: forall x:nat, x = 1 -> (forall a y z:nat, a = 1 -> y = 1 -> z+y+a = 2 -> z+1 = x -> False) -> x > 1.
+  Proof.
+    intros x hx h_eqone.
+    especialize h_eqone with a at 1 .
+    + reflexivity.
+    + exfalso.
+      apply h_eqone with 1 0.
+      * reflexivity.
+      * reflexivity.
+      * symmetry.
+        assumption.
+  Qed.
+  Lemma test_espec6_h: forall x:nat, x = 1 -> (forall a y z:nat, a = 1 -> y = 1 -> z+y+a = 2 -> z+1 = x -> False) -> x > 1.
+  Proof.
+    intros x hx h_eqone.
+    especialize h_eqone with a at 1 as h.
+    + reflexivity.
+    + exfalso.
+      apply h with 1 0.
+      * reflexivity.
+      * reflexivity.
+      * symmetry.
+        assumption.
+  Qed.
+  Lemma test_espec6_h2: forall x:nat, x = 1 -> (forall a y z:nat, a = 1 -> y = 1 -> z+y+a = 2 -> z+1 = x -> False) -> x > 1.
+  Proof.
+    intros x hx h_eqone.
+    especialize h_eqone with a at 1 as ?.
+    + reflexivity.
+    + exfalso.
+      apply H with 1 0.
+      * reflexivity.
+      * reflexivity.
+      * symmetry.
+        assumption.
+  Qed.
 
-  especialize (let x:=Nat.le_antisymm in x) as ? at 2 : h;
-    [ admit |
-      match type of H_spec with (_ <= _ -> _ = _) => idtac | _ => fail "Test failed!" end;
-      match type of h with _ <= _ => idtac | _ => fail "Test failed!" end].
-  Undo.
+  Lemma test_espec7: forall x:nat, x = 1 -> (forall a y z:nat, a = 1 -> y = 1 -> z+y+a = 2 -> z+1 = x -> False) -> x > 1.
+  Proof.
+    intros x hx h_eqone.
+    especialize h_eqone with a,z at 1,4 .
+    + reflexivity.
+    + rewrite hx.
+      instantiate (z:=0).
+      reflexivity.
+    + exfalso.
+      apply h_eqone with 1.
+      * reflexivity.
+      * reflexivity.
+  Qed.
 
-  especialize h_eqone at 2 as ? : ? ;
-    [ admit | match type of h_eqone_spec with eq_one 2 -> eq_one 1 -> False => idtac | _ => fail "Test failed!" end;
-              match type of h_eqone_prem with 3=1 => idtac | _ => fail "Test failed!" end].
-  Undo.
+  Lemma test_espec7_h: forall x:nat, x = 1 -> (forall a y z:nat, a = 1 -> y = 1 -> z+y+a = 2 -> z+1 = x -> False) -> x > 1.
+  Proof.
+    intros x hx h_eqone.
+    especialize h_eqone with a,z at 1,4 as h.
+    + reflexivity.
+    + rewrite hx.
+      instantiate (z:=0).
+      reflexivity.
+    + exfalso.
+      apply h with 1.
+      * reflexivity.
+      * reflexivity.
+  Qed.
+  Lemma test_espec7_h2: forall x:nat, x = 1 -> (forall a y z:nat, a = 1 -> y = 1 -> z+y+a = 2 -> z+1 = x -> False) -> x > 1.
+  Proof.
+    intros x hx h_eqone.
+    especialize h_eqone with a,z at 1,4 as ?.
+    + reflexivity.
+    + rewrite hx.
+      instantiate (z:=0).
+      reflexivity.
+    + exfalso.
+      apply H with 1.
+      * reflexivity.
+      * reflexivity.
+  Qed.
 
-  especialize (let x:=Nat.le_antisymm in x) at 2 as ? : ? ;
-    [ admit |
-      match type of H_spec with (_ <= _ -> _ = _) => idtac | _ => fail "Test failed!" end;
-      match type of H_prem with _ <= _ => idtac | _ => fail "Test failed!" end].
-  Undo.
+  Lemma test_espec8: forall x:nat, x = 1 -> (forall a y z:nat, a = 1 -> y = 1 -> z+y+a = 2 -> z+1 = x -> False) -> x > 1.
+  Proof.
+    intros x hx h_eqone.
+    Fail especialize h_eqone with a at 1,4 .
+  Abort.
 
-  especialize h_eqone as ? at 2 : ? ;
-    [ admit | match goal with h_eqone_spec:eq_one 2 -> eq_one 1 -> False,
-                              h_eqone_prem : 3 = 1 |- _ => idtac | _ => fail "Test failed!" end].
-  Undo.
+  Lemma test_espec8_h: forall x:nat, x = 1 -> (forall a y z:nat, a = 1 -> y = 1 -> z+y+a = 2 -> z+1 = x -> False) -> x > 1.
+  Proof.
+    intros x hx h_eqone.
+    Fail especialize h_eqone with a at 1,4 as h.
+  Abort.
 
-  especialize (let x:=Nat.le_antisymm in x) as ? at 2 : ? ;
-    [ admit |
-      match type of H_spec with (_ <= _ -> _ = _) => idtac | _ => fail "Test failed!" end;
-      match type of H_prem with _ <= _ => idtac | _ => fail "Test failed!" end].
-  Undo.
+  Lemma test_espec8_h: forall x:nat, x = 1 -> (forall a y z:nat, a = 1 -> y = 1 -> z+y+a = 2 -> z+1 = x -> False) -> x > 1.
+  Proof.
+    intros x hx h_eqone.
+    Fail especialize h_eqone with a at 1,4 as ?.
+  Abort.
 
-  especialize h_eqone at 2,3;
-    [ admit | admit| match type of h_eqone with eq_one 2 -> False=> idtac | _ => fail "Test failed!" end].
-  Undo.
+  Lemma test_espec9: forall x:nat, x = 1 -> (forall a y z:nat, a = 1 -> y = 1 -> z+y+a = 2 -> z+1 = x -> False) -> x > 1.
+  Proof.
+    intros x hx h_eqone.
+    Fail especialize h_eqone at 1,4.
+  Abort.
 
-  especialize (let x:=Nat.le_antisymm in x) at 1,2;
-    [ admit | admit | match goal with |- (_ = _) -> True => idtac | _ => fail "Test failed!" end].
-  Undo.
+  Lemma test_espec9_h: forall x:nat, x = 1 -> (forall a y z:nat, a = 1 -> y = 1 -> z+y+a = 2 -> z+1 = x -> False) -> x > 1.
+  Proof.
+    intros x hx h_eqone.
+    Fail especialize h_eqone at 1,4 as h.
+  Abort.
 
-  especialize h_eqone at 3,2;
-    [ admit | admit| match type of h_eqone with eq_one 2 -> False=> idtac | _ => fail "Test failed!" end].
-  Undo.
+  Lemma test_espec9_h: forall x:nat, x = 1 -> (forall a y z:nat, a = 1 -> y = 1 -> z+y+a = 2 -> z+1 = x -> False) -> x > 1.
+  Proof.
+    intros x hx h_eqone.
+    Fail especialize h_eqone at 1,4 as ?.
+  Abort.
 
-  especialize (let x:=Nat.le_antisymm in x) at 2,1;
-    [ admit | admit | match goal with |- (_ = _) -> True => idtac | _ => fail "Test failed!" end].
-  Undo.
+End Using.
 
-  especialize h_eqone as h at 2,3;
-    [ admit | admit| match type of h with eq_one 2 -> False=> idtac | _ => fail "Test failed!" end].
-  Undo.
 
-  especialize (let x:=Nat.le_antisymm in x) at 2,1 as h;
-    [ admit | admit | 
-      match type of h with (_ = _) => idtac | _ => fail "Test failed!" end].
-  Undo.
-
-  especialize h_eqone at 2,3 as h;
-    [ admit | admit| match type of h with eq_one 2 -> False=> idtac | _ => fail "Test failed!" end].
-  Undo.
-
-  especialize (let x:=Nat.le_antisymm in x) as h at 2,1;
-    [ admit | admit | 
-      match type of h with (_ = _) => idtac | _ => fail "Test failed!" end].
-  Undo.
-
-  especialize h_eqone at 3,2,1;
-    [ admit | admit | admit |  match type of h_eqone with False=> idtac | _ => fail "Test failed!" end ].
-  Undo.
-
-  especialize h_eqone as h at 3,2,1;
-    [ admit | admit | admit |  match type of h with False=> idtac | _ => fail "Test failed!" end ].
-  Undo.
-
-  especialize h_eqone at 3,2,1 as h;
-    [ admit | admit | admit |  match type of h with False=> idtac | _ => fail "Test failed!" end ].
-  Undo.
-  exact I.
-Qed.
-
-Lemma foo2: (eq_one 2 -> eq_one 3 ->eq_one 4 ->eq_one 5 ->eq_one 6 -> eq_one 1 -> False) -> True.
+Lemma test_esepec_6_7: (eq_one 2 -> eq_one 3 ->eq_one 4 ->eq_one 5 ->eq_one 6 ->eq_one 7 ->eq_one 8 -> eq_one 9 -> eq_one 1 -> False) -> True.
 Proof.
-  intros h_eqone.
-  especialize h_eqone at 3,1,4,5 as h;
-    [ admit | admit | admit  | admit | match type of h with eq_one 3 -> eq_one 1 ->False=> idtac | _ => fail "Test failed!" end  ]. 
+  intros H.
+  especialize H at 3,1,4,5,2,7 as h; [ admit | admit | admit  | admit | admit | admit | match type of h with eq_one 7 -> eq_one 9 -> eq_one 1 ->False=> idtac "OK" end].
   Undo.
-  especialize h_eqone as h at 3,1,4,5;
-    [ admit | admit | admit  | admit | match type of h with eq_one 3 -> eq_one 1 ->False=> idtac | _ => fail "Test failed!" end  ]. 
+  especialize H at 3,1,4,5,2,7; [ admit | admit | admit  | admit | admit | admit | match type of H with eq_one 7 -> eq_one 9 -> eq_one 1 ->False=> idtac "OK" end].
   Undo.
-  especialize h_eqone at 3,1,4,5;
-    [ admit | admit | admit  | admit | match type of h_eqone with eq_one 3 -> eq_one 1 ->False=> idtac | _ => fail "Test failed!" end  ]. 
+  especialize H at 3,1,4,5,2,7,9 as h; [ admit | admit | admit  | admit | admit | admit | admit | match type of h with eq_one 7 -> eq_one 9 -> False => idtac "OK" end].
   Undo.
-  especialize h_eqone at 3,1,4,5,2;
-    [ admit | admit | admit | admit  | admit | match type of h_eqone with eq_one 1 ->False=> idtac | _ => fail "Test failed!" end  ]. 
-  Undo.
-  especialize h_eqone at 3,1,4,5,2  as h;
-    [ admit | admit | admit | admit  | admit | match type of h with eq_one 1 ->False=> idtac | _ => fail "Test failed!" end  ]. 
-  Undo.
-  especialize h_eqone as h at 3,1,4,5,2;
-    [ admit | admit | admit | admit  | admit | match type of h with eq_one 1 ->False=> idtac | _ => fail "Test failed!" end  ]. 
+  especialize H at 3,1,4,5,2,7,9; [ admit | admit | admit  | admit | admit | admit | admit | match type of H with eq_one 7 -> eq_one 9 -> False => idtac "OK" end].
   Undo.
   exact I.
 Qed.
+
+
+Axiom ex_hyp : (forall (b:bool), forall x: nat, eq_one 1 -> forall y:nat, eq_one 2 ->eq_one 3 ->eq_one 4 ->eq_one x ->eq_one 6 ->eq_one y -> eq_one 8 -> eq_one 9 -> False).
+
+Lemma test_esepec: True.
+Proof.
+
+  especialize (ex_hyp true) at 2 as h;[ .. | match type of h with forall x: nat, eq_one 1 -> forall y:nat, eq_one 3 -> eq_one 4 -> eq_one _ -> eq_one 6 -> eq_one _ -> eq_one 8 -> eq_one 9 -> False => idtac "OK" end].
+  Undo.
+  especialize (ex_hyp true) at 2,3 as h;[  .. | match type of h with forall x: nat, eq_one 1 -> forall y:nat, eq_one 4 -> eq_one _ -> eq_one 6 -> eq_one _ -> eq_one 8 -> eq_one 9 -> False => idtac "OK" end].
+  Undo.
+  Fail especialize H at 2,3,5 as h. 
+  Undo.
+  especialize (ex_hyp true) with x at 2,3,5 as h ;[ ..  | match type of h with eq_one 1 -> forall y:nat, eq_one 4 -> eq_one 6 -> eq_one _ -> eq_one 8 -> eq_one 9 -> False => idtac "OK" end].
+  Undo.
+  especialize (ex_hyp true) with x at 2,3,5,6 as h ;[ ..  | match type of h with eq_one 1 -> forall y:nat, eq_one 4 -> eq_one _ -> eq_one 8 -> eq_one 9 -> False => idtac "OK" end].
+  Undo.
+  Fail especialize H with x at 2,3,5,7 as h.
+  especialize (ex_hyp true) with x,y at 2,3,5,7 as h ;[ ..  | match type of h with eq_one 1 -> eq_one 4 -> eq_one 6 -> eq_one 8 -> eq_one 9 -> False => idtac "OK" end].
+  Undo.
+  especialize (ex_hyp true) with x,y at 2,3,5,7,9 as h ;[ ..  | match type of h with eq_one 1 -> eq_one 4 -> eq_one 6 -> eq_one 8 -> False => idtac "OK" end].
+  Undo.
+  especialize (ex_hyp true) with x,y at 2,3,1,5,7,9 as h ;[ ..  | match type of h with eq_one 4 -> eq_one 6 -> eq_one 8 -> False => idtac "OK" end].
+  Undo.
+  especialize (ex_hyp true) with x,y at 8,2,3,5,7,9 as h ;[ ..  | match type of h with eq_one 1 -> eq_one 4 -> eq_one 6 -> False => idtac "OK" end].
+  Undo.
+
+  especialize (ex_hyp true) at 2 as ?;[ .. | match type of H with forall x: nat, eq_one 1 -> forall y:nat, eq_one 3 -> eq_one 4 -> eq_one _ -> eq_one 6 -> eq_one _ -> eq_one 8 -> eq_one 9 -> False => idtac "OK" end].
+  Undo.
+  especialize (ex_hyp true) at 2,3 as ?;[  .. | match type of H with forall x: nat, eq_one 1 -> forall y:nat, eq_one 4 -> eq_one _ -> eq_one 6 -> eq_one _ -> eq_one 8 -> eq_one 9 -> False => idtac "OK" end].
+  Undo.
+  Fail especialize H at 2,3,5 as ?. 
+  Undo.
+  especialize (ex_hyp true) with x at 2,3,5 as ? ;[ ..  | match type of H with eq_one 1 -> forall y:nat, eq_one 4 -> eq_one 6 -> eq_one _ -> eq_one 8 -> eq_one 9 -> False => idtac "OK" end].
+  Undo.
+  especialize (ex_hyp true) with x at 2,3,5,6 as ? ;[ ..  | match type of H with eq_one 1 -> forall y:nat, eq_one 4 -> eq_one _ -> eq_one 8 -> eq_one 9 -> False => idtac "OK" end].
+  Undo.
+  Fail especialize H with x at 2,3,5,7 as ?.
+  especialize (ex_hyp true) with x,y at 2,3,5,7 as ? ;[ ..  | match type of H with eq_one 1 -> eq_one 4 -> eq_one 6 -> eq_one 8 -> eq_one 9 -> False => idtac "OK" end].
+  Undo.
+  especialize (ex_hyp true) with x,y at 2,3,5,7,9 as ? ;[ ..  | match type of H with eq_one 1 -> eq_one 4 -> eq_one 6 -> eq_one 8 -> False => idtac "OK" end].
+  Undo.
+  especialize (ex_hyp true) with x,y at 2,3,1,5,7,9 as ? ;[ ..  | match type of H with eq_one 4 -> eq_one 6 -> eq_one 8 -> False => idtac "OK" end].
+  Undo.
+  especialize (ex_hyp true) with x,y at 8,2,3,5,7,9 as ? ;[ ..  | match type of H with eq_one 1 -> eq_one 4 -> eq_one 6 -> False => idtac "OK" end].
+  Undo.
+
+  Fail especialize (ex_hyp true) at 2.
+
+  Undo.
+  generalize (ex_hyp true) as H.
+  intro.
+  especialize H at 2 as h;[ .. | match type of h with forall x: nat, eq_one 1 -> forall y:nat, eq_one 3 -> eq_one 4 -> eq_one _ -> eq_one 6 -> eq_one _ -> eq_one 8 -> eq_one 9 -> False => idtac "OK" end].
+  Undo.
+  especialize H at 2,3 as h;[  .. | match type of h with forall x: nat, eq_one 1 -> forall y:nat, eq_one 4 -> eq_one _ -> eq_one 6 -> eq_one _ -> eq_one 8 -> eq_one 9 -> False => idtac "OK" end].
+  Undo.
+  Fail especialize H at 2,3,5 as h. 
+  Undo.
+  especialize H with x at 2,3,5 as h ;[ ..  | match type of h with eq_one 1 -> forall y:nat, eq_one 4 -> eq_one 6 -> eq_one _ -> eq_one 8 -> eq_one 9 -> False => idtac "OK" end].
+  Undo.
+  especialize H with x at 2,3,5,6 as h ;[ ..  | match type of h with eq_one 1 -> forall y:nat, eq_one 4 -> eq_one _ -> eq_one 8 -> eq_one 9 -> False => idtac "OK" end].
+  Undo.
+  Fail especialize H with x at 2,3,5,7 as h.
+  especialize H with x,y at 2,3,5,7 as h ;[ ..  | match type of h with eq_one 1 -> eq_one 4 -> eq_one 6 -> eq_one 8 -> eq_one 9 -> False => idtac "OK" end].
+  Undo.
+  especialize H with x,y at 2,3,5,7,9 as h ;[ ..  | match type of h with eq_one 1 -> eq_one 4 -> eq_one 6 -> eq_one 8 -> False => idtac "OK" end].
+  Undo.
+  especialize H with x,y at 2,3,1,5,7,9 as h ;[ ..  | match type of h with eq_one 4 -> eq_one 6 -> eq_one 8 -> False => idtac "OK" end].
+  Undo.
+  especialize H with x,y at 8,2,3,5,7,9 as h ;[ ..  | match type of h with eq_one 1 -> eq_one 4 -> eq_one 6 -> False => idtac "OK" end].
+  Undo.
+
+  especialize H at 2 as ?;[ .. | match type of H0 with forall x: nat, eq_one 1 -> forall y:nat, eq_one 3 -> eq_one 4 -> eq_one _ -> eq_one 6 -> eq_one _ -> eq_one 8 -> eq_one 9 -> False => idtac "OK" end].
+  Undo.
+  especialize H at 2,3 as ?;[  .. | match type of H0 with forall x: nat, eq_one 1 -> forall y:nat, eq_one 4 -> eq_one _ -> eq_one 6 -> eq_one _ -> eq_one 8 -> eq_one 9 -> False => idtac "OK" end].
+  Undo.
+  Fail especialize H at 2,3,5 as ?. 
+  Undo.
+  especialize H with x at 2,3,5 as ? ;[ ..  | match type of H0 with eq_one 1 -> forall y:nat, eq_one 4 -> eq_one 6 -> eq_one _ -> eq_one 8 -> eq_one 9 -> False => idtac "OK" end].
+  Undo.
+  especialize H with x at 2,3,5,6 as ? ;[ ..  | match type of H0 with eq_one 1 -> forall y:nat, eq_one 4 -> eq_one _ -> eq_one 8 -> eq_one 9 -> False => idtac "OK" end].
+  Undo.
+  Fail especialize H with x at 2,3,5,7 as ?.
+  especialize H with x,y at 2,3,5,7 as ? ;[ ..  | match type of H0 with eq_one 1 -> eq_one 4 -> eq_one 6 -> eq_one 8 -> eq_one 9 -> False => idtac "OK" end].
+  Undo.
+  especialize H with x,y at 2,3,5,7,9 as ? ;[ ..  | match type of H0 with eq_one 1 -> eq_one 4 -> eq_one 6 -> eq_one 8 -> False => idtac "OK" end].
+  Undo.
+  especialize H with x,y at 2,3,1,5,7,9 as ? ;[ ..  | match type of H0 with eq_one 4 -> eq_one 6 -> eq_one 8 -> False => idtac "OK" end].
+  Undo.
+  especialize H with x,y at 8,2,3,5,7,9 as ? ;[ ..  | match type of H0 with eq_one 1 -> eq_one 4 -> eq_one 6 -> False => idtac "OK" end].
+  Undo.
+
+  especialize H at 2;[ .. | match type of H with forall x: nat, eq_one 1 -> forall y:nat, eq_one 3 -> eq_one 4 -> eq_one _ -> eq_one 6 -> eq_one _ -> eq_one 8 -> eq_one 9 -> False => idtac "OK" end].
+  Undo.
+  especialize H at 2,3;[  .. | match type of H with forall x: nat, eq_one 1 -> forall y:nat, eq_one 4 -> eq_one _ -> eq_one 6 -> eq_one _ -> eq_one 8 -> eq_one 9 -> False => idtac "OK" end].
+  Undo.
+  Fail especialize H at 2,3,5. 
+  Undo.
+  especialize H with x at 2,3,5 ;[ ..  | match type of H with eq_one 1 -> forall y:nat, eq_one 4 -> eq_one 6 -> eq_one _ -> eq_one 8 -> eq_one 9 -> False => idtac "OK" end].
+  Undo.
+  especialize H with x at 2,3,5,6 ;[ ..  | match type of H with eq_one 1 -> forall y:nat, eq_one 4 -> eq_one _ -> eq_one 8 -> eq_one 9 -> False => idtac "OK" end].
+  Undo.
+  Fail especialize H with x at 2,3,5,7.
+  especialize H with x,y at 2,3,5,7 ;[ ..  | match type of H with eq_one 1 -> eq_one 4 -> eq_one 6 -> eq_one 8 -> eq_one 9 -> False => idtac "OK" end].
+  Undo.
+  especialize H with x,y at 2,3,5,7,9 ;[ ..  | match type of H with eq_one 1 -> eq_one 4 -> eq_one 6 -> eq_one 8 -> False => idtac "OK" end].
+  Undo.
+  especialize H with x,y at 2,3,1,5,7,9 ;[ ..  | match type of H with eq_one 4 -> eq_one 6 -> eq_one 8 -> False => idtac "OK" end].
+  Undo.
+  especialize H with x,y at 8,2,3,5,7,9 ;[ ..  | match type of H with eq_one 1 -> eq_one 4 -> eq_one 6 -> False => idtac "OK" end].
+  Undo.
+
+  exact I.
+Qed.
+
 
 
 Lemma test_espec_namings: forall n:nat, (eq_one n -> eq_one 1 -> False) -> True.
 Proof.
   intros n h_eqone.
-  especialize Nat.quadmul_le_squareadd at 1 as hh : h.
+  especialize Nat.quadmul_le_squareadd with a at 1 as hh : h.
   { apply le_n. }
-  especialize min_l at 1 as ? : ?.
+  especialize min_l with n,m at 1 as ?.
   { apply (le_n O). }
   especialize h_eqone at 2 as h1 : h2.
   { reflexivity. }
+  unfold eq_one in h2.
   match type of h2 with 1 = 1 => idtac | _ => fail end.
   match type of h1 with eq_one n -> False => idtac | _ => fail end.
   exact I.
 Qed.
 
-Lemma test_esepec_6_7: (eq_one 2 -> eq_one 3 ->eq_one 4 ->eq_one 5 ->eq_one 6 ->eq_one 7 ->eq_one 8 -> eq_one 9 -> eq_one 1 -> False) -> True.
-Proof.
-  intros h_eqone.
-  especialize h_eqone at 3,1,4,5,2,7 as h;
-    [ admit | admit | admit  | admit | admit | admit | match type of h with eq_one 7 -> eq_one 9 -> eq_one 1 ->False=> idtac | _ => fail "Test failed!" end].
-  Undo.
-  especialize h_eqone as h at 3,1,4,5,2,7;
-    [ admit | admit | admit  | admit | admit | admit | match type of h with eq_one 7 -> eq_one 9 -> eq_one 1 ->False=> idtac | _ => fail "Test failed!" end].
-  Undo.
-  especialize h_eqone at 3,1,4,5,2,7;
-    [ admit | admit | admit  | admit | admit | admit | match type of h_eqone with eq_one 7 -> eq_one 9 -> eq_one 1 ->False=> idtac | _ => fail "Test failed!" end].
-  Undo.
-  especialize h_eqone at 3,1,4,5,2,7,9 as h;
-    [ admit | admit | admit  | admit | admit | admit | admit | match type of h with eq_one 7 -> eq_one 9 -> False => idtac | _ => fail "Test failed!" end].
-  Undo.
-  especialize h_eqone as h at 3,1,4,5,2,7,9;
-    [ admit | admit | admit  | admit | admit | admit | admit | match type of h with eq_one 7 -> eq_one 9 -> False => idtac | _ => fail "Test failed!" end].
-  Undo.
-  especialize h_eqone at 3,1,4,5,2,7,9;
-    [ admit | admit | admit  | admit | admit | admit | admit | match type of h_eqone with eq_one 7 -> eq_one 9 -> False => idtac | _ => fail "Test failed!" end].
-  Undo.
-  exact I.
-Qed.
 
 (* "until i" and "at *" *)
 
@@ -375,14 +679,26 @@ Proof.
   
   intros h_eqone.
   (* specialize on term ==> create a new hyp *)
-  especialize (let x:=not_eq_S in x) at *;
-    [ intro ; admit | match type of H_spec with (S _)<>(S _) => idtac | _ => fail "Test failed!" end].
+
+  Fail especialize (let x:=not_eq_S in x) with n,m at *.
+  especialize (let x:=not_eq_S in x) with n,m at * as h;
+    [ .. | match type of h with (S _)<>(S _) => idtac | _ => fail "Test failed!" end].
   Undo.
-  especialize (let x:=not_eq_S in x) at * as h;
-    [ intro ; admit | match type of h with (S _)<>(S _) => idtac | _ => fail "Test failed!" end].
+  especialize (let x:=not_eq_S in x) with n,m at * as ?;
+    [ .. | match type of H with (S _)<>(S _) => idtac | _ => fail "Test failed!" end].
+  Undo.
+  Fail especialize (let x:=not_eq_S in x) with n,m until 1.
+  especialize (let x:=not_eq_S in x) with n,m at * as h;
+    [ .. | match type of h with (S _)<>(S _) => idtac | _ => fail "Test failed!" end].
+  Undo.
+  especialize (let x:=Nat.sub_pred_r in x) with n,m until 2 as h;
+    [ .. | match type of h with ?n - Nat.pred ?m = S (?n - ?m) => idtac | _ => fail "Test failed!" end].
+  Undo.
+  especialize (let x:=Nat.sub_pred_r in x) with n,m until 1 as h;
+    [ .. | match type of h with ?m <= ?n -> ?n - Nat.pred ?m = S (?n - ?m) => idtac | _ => fail "Test failed!" end].
   Undo.
   especialize (let x:=h_eqone in x) at *;
-    [ admit |admit |admit |admit |admit |admit |admit |admit |admit | match type of H_spec with False => idtac | _ => fail "Test failed!" end].
+    [ ..  | match type of H_spec with False => idtac | _ => fail "Test failed!" end].
   Undo.
   (* proveprem_until h_eqone 4. *)
   especialize (let x:= h_eqone in x) until 4;
@@ -393,7 +709,7 @@ Proof.
     [ admit |admit |admit |admit | match type of h_eqone with eq_one 6 -> eq_one 7 -> eq_one 8 -> eq_one 9 -> eq_one 1 -> False => idtac | _ => fail "Test failed!" end].
   Undo.
   especialize h_eqone at * ;
-    [ admit |admit |admit |admit |admit |admit |admit |admit |admit | match type of h_eqone with False => idtac | _ => fail "Test failed!" end].
+    [ .. | match type of h_eqone with False => idtac | _ => fail "Test failed!" end].
   Undo.
   (* unless we give the "as" option *)
   especialize h_eqone at * as h ;
@@ -405,7 +721,6 @@ Proof.
   Undo.
   exact I.
 Qed.
-*)
 
 Require Import LibHyps.LibDecomp.
 
